theories/Eq/SSim0Theory.v
@@ -35,27 +35,27 @@ Import CTreeNotations.
 Import EquNotations.
 Import SBisimNotations.
 
-Section ssim0_homogenous_theory.
+Section ssim_homogenous_theory.
   Context {E C: Type -> Type} {X: Type}
           {L: relation (@label E)}
           {HasStuck1: B0 -< C}.
 
-  Notation ss0 := (@ss0 E E C C X X _ _).
-  Notation ssim0 := (@ssim0 E E C C X X _ _).
-  Notation sst0 L := (coinduction.t (ss0 L)).
-  Notation ssbt0 L := (coinduction.bt (ss0 L)).
-  Notation ssT0 L := (coinduction.T (ss0 L)).
+  Notation ss := (@ss E E C C X X _ _).
+  Notation ssim := (@ssim E E C C X X _ _).
+  Notation sst L := (coinduction.t (ss L)).
+  Notation ssbt L := (coinduction.bt (ss L)).
+  Notation ssT L := (coinduction.T (ss L)).
 
   (*|
     Various results on reflexivity and transitivity.
   |*)
-  Lemma refl_sst0 `{Reflexive _ L}: const seq <= (sst0 L).
+  Lemma refl_sst `{Reflexive _ L}: const seq <= (sst L).
   Proof.
     apply leq_t. cbn.
     intros. unfold seq in H0. subst. eauto.
   Qed.
 
-  Lemma square_sst0 `{Transitive _ L}: square <= (sst0 L).
+  Lemma square_sst `{Transitive _ L}: square <= (sst L).
   Proof.
     apply Coinduction; cbn.
     intros R x z [y xy yz] l x' xx'.
@@ -65,48 +65,48 @@ Section ssim0_homogenous_theory.
     split.
     assumption.
     split.
-    apply (f_Tf (ss0 L)).
+    apply (f_Tf (ss L)).
     exists y'; eauto.
     transitivity l'; auto.
   Qed.
 
   (*| Reflexivity |*)
-  #[global] Instance Reflexive_sst0 R `{Reflexive _ L}: Reflexive (sst0 L R).
-  Proof. apply build_reflexive; apply ft_t; apply (refl_sst0). Qed.
+  #[global] Instance Reflexive_sst R `{Reflexive _ L}: Reflexive (sst L R).
+  Proof. apply build_reflexive; apply ft_t; apply (refl_sst). Qed.
 
-  Corollary Reflexive_ssim0 `{Reflexive _ L}: Reflexive (ssim0 L).
-  Proof. now apply Reflexive_sst0. Qed.
+  Corollary Reflexive_ssim `{Reflexive _ L}: Reflexive (ssim L).
+  Proof. now apply Reflexive_sst. Qed.
 
-  #[global] Instance Reflexive_ssbt0 R `{Reflexive _ L}: Reflexive (ssbt0 L R).
-  Proof. apply build_reflexive; apply fbt_bt; apply refl_sst0. Qed.
+  #[global] Instance Reflexive_ssbt R `{Reflexive _ L}: Reflexive (ssbt L R).
+  Proof. apply build_reflexive; apply fbt_bt; apply refl_sst. Qed.
 
-  #[global] Instance Reflexive_ssT0 f R `{Reflexive _ L}: Reflexive (ssT0 L f R).
-  Proof. apply build_reflexive; apply fT_T; apply refl_sst0. Qed.
+  #[global] Instance Reflexive_ssT f R `{Reflexive _ L}: Reflexive (ssT L f R).
+  Proof. apply build_reflexive; apply fT_T; apply refl_sst. Qed.
 
   (*| Transitivity |*)
-  #[global] Instance Transitive_sst0 R `{Transitive _ L}: Transitive (sst0 L R).
-  Proof. apply build_transitive; apply ft_t; apply (square_sst0). Qed.
+  #[global] Instance Transitive_sst R `{Transitive _ L}: Transitive (sst L R).
+  Proof. apply build_transitive; apply ft_t; apply (square_sst). Qed.
 
-  Corollary Transitive_ssim0 `{Transitive _ L}: Transitive (ssim0 L).
-  Proof. now apply Transitive_sst0. Qed.
+  Corollary Transitive_ssim `{Transitive _ L}: Transitive (ssim L).
+  Proof. now apply Transitive_sst. Qed.
 
-  #[global] Instance Transitive_ssbt0 R `{Transitive _ L}: Transitive (ssbt0 L R).
-  Proof. apply build_transitive; apply fbt_bt; apply square_sst0. Qed.
+  #[global] Instance Transitive_ssbt R `{Transitive _ L}: Transitive (ssbt L R).
+  Proof. apply build_transitive; apply fbt_bt; apply square_sst. Qed.
 
-  #[global] Instance Transitive_ssT0 f R `{Transitive _ L}: Transitive (ssT0 L f R).
-  Proof. apply build_transitive; apply fT_T; apply square_sst0. Qed.
+  #[global] Instance Transitive_ssT f R `{Transitive _ L}: Transitive (ssT L f R).
+  Proof. apply build_transitive; apply fT_T; apply square_sst. Qed.
 
   (*| PreOrder |*)
-  #[global] Instance PreOrder_sst0 R `{PreOrder _ L}: PreOrder (sst0 L R).
+  #[global] Instance PreOrder_sst R `{PreOrder _ L}: PreOrder (sst L R).
   Proof. split; typeclasses eauto. Qed.
 
-  Corollary PreOrder_ssim0 `{PreOrder _ L}: PreOrder (ssim0 L).
+  Corollary PreOrder_ssim `{PreOrder _ L}: PreOrder (ssim L).
   Proof. split; typeclasses eauto. Qed.
 
-  #[global] Instance PreOrder_ssbt0 R `{PreOrder _ L}: PreOrder (ssbt0 L R).
+  #[global] Instance PreOrder_ssbt R `{PreOrder _ L}: PreOrder (ssbt L R).
   Proof. split; typeclasses eauto. Qed.
 
-  #[global] Instance PreOrder_ssT0 f R `{PreOrder _ L}: PreOrder (ssT0 L f R).
+  #[global] Instance PreOrder_ssT f R `{PreOrder _ L}: PreOrder (ssT L f R).
   Proof. split; typeclasses eauto. Qed.
 
   (*|
@@ -114,33 +114,33 @@ Section ssim0_homogenous_theory.
     [sbisim] under all [ss1]-related contexts (consequence of the transitivity
     of the companion).
     |*)
-  #[global] Instance sbisim_clos_ssim0_goal `{Symmetric _ L} `{Transitive _ L} :
-    Proper (sbisim L ==> sbisim L ==> flip impl) (ssim0 L).
+  #[global] Instance sbisim_clos_ssim_goal `{Symmetric _ L} `{Transitive _ L} :
+    Proper (sbisim L ==> sbisim L ==> flip impl) (ssim L).
   Proof.
     repeat intro.
     transitivity y0. transitivity y.
-    - now apply sbisim_ssim0 in H1.
+    - now apply sbisim_ssim in H1.
     - now exact H3.
-    - symmetry in H2; now apply sbisim_ssim0 in H2.
+    - symmetry in H2; now apply sbisim_ssim in H2.
   Qed.
 
-  #[global] Instance sbisim_clos_ssim0_ctx `{Equivalence _ L}:
-    Proper (sbisim L ==> sbisim L ==> impl) (ssim0 L).
+  #[global] Instance sbisim_clos_ssim_ctx `{Equivalence _ L}:
+    Proper (sbisim L ==> sbisim L ==> impl) (ssim L).
   Proof.
-    repeat intro. symmetry in H0, H1. eapply sbisim_clos_ssim0_goal; eauto.
+    repeat intro. symmetry in H0, H1. eapply sbisim_clos_ssim_goal; eauto.
   Qed.
 
   #[global] Instance sbisim_clos_sst_goal RR `{Equivalence _ L}:
-    Proper (sbisim L ==> sbisim L ==> flip impl) (sst0 L RR).
+    Proper (sbisim L ==> sbisim L ==> flip impl) (sst L RR).
   Proof.
     cbn; intros ? ? eq1 ? ? eq2 H0.
-    symmetry in eq2. apply sbisim_ssim0 in eq1, eq2.
+    symmetry in eq2. apply sbisim_ssim in eq1, eq2.
     rewrite eq1, <- eq2.
     auto.
   Qed.
 
   #[global] Instance sbisim_clos_sst_ctx RR `{Equivalence _ L}:
-    Proper (sbisim L ==> sbisim L ==> impl) (sst0 L RR).
+    Proper (sbisim L ==> sbisim L ==> impl) (sst L RR).
   Proof.
     cbn; intros ? ? eq1 ? ? eq2 ?.
     rewrite <- eq1, <- eq2.
@@ -148,42 +148,42 @@ Section ssim0_homogenous_theory.
   Qed.
 
   #[global] Instance sbisim_clos_ssT_goal RR f `{Equivalence _ L}:
-    Proper (sbisim L ==> sbisim L ==> flip impl) (ssT0 L f RR).
+    Proper (sbisim L ==> sbisim L ==> flip impl) (ssT L f RR).
   Proof.
     cbn; intros ? ? eq1 ? ? eq2 ?.
-    symmetry in eq2. apply sbisim_ssim0 in eq1, eq2.
+    symmetry in eq2. apply sbisim_ssim in eq1, eq2.
     rewrite eq1, <- eq2.
     auto.
   Qed.
 
   #[global] Instance sbisim_clos_ssT_ctx RR f `{Equivalence _ L}:
-    Proper (sbisim L ==> sbisim L ==> impl) (ssT0 L f RR).
+    Proper (sbisim L ==> sbisim L ==> impl) (ssT L f RR).
   Proof.
     cbn; intros ? ? eq1 ? ? eq2 ?.
     rewrite <- eq1, <- eq2.
     auto.
   Qed.
 
-End ssim0_homogenous_theory.
+End ssim_homogenous_theory.
 
-(*| Parametric theory of [ss0] with heterogenous [L] |*)
-Section ssim0_heterogenous_theory.
+(*| Parametric theory of [ss] with heterogenous [L] |*)
+Section ssim_heterogenous_theory.
   Arguments label: clear implicits.
   Context {E F C D: Type -> Type} {X Y: Type}
           {L: rel (@label E) (@label F)}
           {HasStuck1: B0 -< C} {HasStuck2: B0 -< D}.
 
-  Notation ss0 := (@ss0 E F C D X Y _ _).
-  Notation ssim0  := (@ssim0 E F C D X Y _ _).
-  Notation sst0 L := (coinduction.t (ss0 L)).
-  Notation ssbt0 L := (coinduction.bt (ss0 L)).
-  Notation ssT0 L := (coinduction.T (ss0 L)).
+  Notation ss := (@ss E F C D X Y _ _).
+  Notation ssim  := (@ssim E F C D X Y _ _).
+  Notation sst L := (coinduction.t (ss L)).
+  Notation ssbt L := (coinduction.bt (ss L)).
+  Notation ssT L := (coinduction.T (ss L)).
 
   (*|
    Strong simulation up-to [equ] is valid
    ----------------------------------------
   |*)
-  Lemma equ_clos_sst0 : equ_clos <= (sst0 L).
+  Lemma equ_clos_sst : equ_clos <= (sst L).
   Proof.
     apply Coinduction; cbn.
     intros R x y [x' y' x'' y'' EQ' EQ''] l z x'z.
@@ -193,77 +193,77 @@ Section ssim0_heterogenous_theory.
     split.
     - rewrite <- Equu; auto.
     - split; auto.
-      eapply (f_Tf (ss0 L)).
+      eapply (f_Tf (ss L)).
       econstructor; auto; auto.
   Qed.
 
-  #[global] Instance equ_clos_sst0_goal {RR} :
-    Proper (equ eq ==> equ eq ==> flip impl) (sst0 L RR).
+  #[global] Instance equ_clos_sst_goal {RR} :
+    Proper (equ eq ==> equ eq ==> flip impl) (sst L RR).
   Proof.
     cbn; intros ? ? eq1 ? ? eq2 H.
-    apply (ft_t equ_clos_sst0); econstructor; [eauto | | symmetry; eauto]; assumption.
+    apply (ft_t equ_clos_sst); econstructor; [eauto | | symmetry; eauto]; assumption.
   Qed.
 
-  #[global] Instance equ_clos_sst0_ctx {RR} :
-    Proper (equ eq ==> equ eq ==> impl) (sst0 L RR).
+  #[global] Instance equ_clos_sst_ctx {RR} :
+    Proper (equ eq ==> equ eq ==> impl) (sst L RR).
   Proof.
     cbn; intros ? ? eq1 ? ? eq2 H.
-    apply (ft_t equ_clos_sst0); econstructor; [symmetry; eauto | | eauto]; assumption.
+    apply (ft_t equ_clos_sst); econstructor; [symmetry; eauto | | eauto]; assumption.
   Qed.
 
-  #[global] Instance equ_ssbt0_closed_goal {r} :
-    Proper (equ eq ==> equ eq ==> flip impl) (ssbt0 L r).
+  #[global] Instance equ_ssbt_closed_goal {r} :
+    Proper (equ eq ==> equ eq ==> flip impl) (ssbt L r).
   Proof.
     cbn. intros.
-    apply (fbt_bt equ_clos_sst0); econstructor; eauto.
+    apply (fbt_bt equ_clos_sst); econstructor; eauto.
     now symmetry.
   Qed.
 
-  #[global] Instance equ_ssbt0_closed_ctx {r} :
-    Proper (equ eq ==> equ eq ==> impl) (ssbt0 L r).
+  #[global] Instance equ_ssbt_closed_ctx {r} :
+    Proper (equ eq ==> equ eq ==> impl) (ssbt L r).
   Proof.
     cbn; intros.
     now rewrite H, H0 in H1.
   Qed.
 
-  #[global] Instance equ_clos_ssT0_goal RR f :
-    Proper (equ eq ==> equ eq ==> flip impl) (ssT0 L f RR).
+  #[global] Instance equ_clos_ssT_goal RR f :
+    Proper (equ eq ==> equ eq ==> flip impl) (ssT L f RR).
   Proof.
     cbn; intros ? ? eq1 ? ? eq2 H.
-    apply (fT_T equ_clos_sst0); econstructor; [eauto | | symmetry; eauto]; assumption.
+    apply (fT_T equ_clos_sst); econstructor; [eauto | | symmetry; eauto]; assumption.
   Qed.
 
-  #[global] Instance equ_clos_ssT0_ctx RR f :
-    Proper (equ eq ==> equ eq ==> impl) (ssT0 L f RR).
+  #[global] Instance equ_clos_ssT_ctx RR f :
+    Proper (equ eq ==> equ eq ==> impl) (ssT L f RR).
   Proof.
     cbn; intros ? ? eq1 ? ? eq2 H.
-    apply (fT_T equ_clos_sst0); econstructor; [symmetry; eauto | | eauto]; assumption.
+    apply (fT_T equ_clos_sst); econstructor; [symmetry; eauto | | eauto]; assumption.
   Qed.
 
-  #[global] Instance equ_clos_ssim0_goal :
-    Proper (equ eq ==> equ eq ==> flip impl) (ssim0 L).
+  #[global] Instance equ_clos_ssim_goal :
+    Proper (equ eq ==> equ eq ==> flip impl) (ssim L).
   Proof.
     cbn; intros ? ? eq1 ? ? eq2 H.
-    apply (ft_t equ_clos_sst0); econstructor; [eauto | | symmetry; eauto]; assumption.
+    apply (ft_t equ_clos_sst); econstructor; [eauto | | symmetry; eauto]; assumption.
   Qed.
 
-  #[global] Instance equ_clos_ssim0_ctx :
-    Proper (equ eq ==> equ eq ==> impl) (ssim0 L).
+  #[global] Instance equ_clos_ssim_ctx :
+    Proper (equ eq ==> equ eq ==> impl) (ssim L).
   Proof.
     cbn; intros ? ? eq1 ? ? eq2 H.
-    apply (ft_t equ_clos_sst0); econstructor; [symmetry; eauto | | eauto]; assumption.
+    apply (ft_t equ_clos_sst); econstructor; [symmetry; eauto | | eauto]; assumption.
   Qed.
 
-  #[global] Instance equ_ss0_closed_goal {r} :
-    Proper (equ eq ==> equ eq ==> flip impl) (ss0 L r).
+  #[global] Instance equ_ss_closed_goal {r} :
+    Proper (equ eq ==> equ eq ==> flip impl) (ss L r).
   Proof.
     intros t t' tt' u u' uu'; cbn; intros.
     rewrite tt' in H0. apply H in H0 as (l' & ? & ? & ? & ?).
     do 2 eexists; eauto. rewrite uu'. eauto.
   Qed.
 
-  #[global] Instance equ_ss0_closed_ctx {r} :
-    Proper (equ eq ==> equ eq ==> impl) (ss0 L r).
+  #[global] Instance equ_ss_closed_ctx {r} :
+    Proper (equ eq ==> equ eq ==> impl) (ss L r).
   Proof.
     intros t t' tt' u u' uu'; cbn; intros.
     rewrite <- tt' in H0. apply H in H0 as (l' & ? & ? & ? & ?).
@@ -273,40 +273,40 @@ Section ssim0_heterogenous_theory.
   (*|
     stuck ctrees can be simulated by anything.
     |*)
-  Lemma is_stuck_ss0 (R : rel _ _) (t : ctree E C X) (t': ctree F D Y):
-    is_stuck t -> ss0 L R t t'.
+  Lemma is_stuck_ss (R : rel _ _) (t : ctree E C X) (t': ctree F D Y):
+    is_stuck t -> ss L R t t'.
   Proof.
     repeat intro. now apply H in H0.
   Qed.
 
-  Lemma is_stuck_ssim0 (t: ctree E C X) (t': ctree F D Y):
-    is_stuck t -> ssim0 L t t'.
+  Lemma is_stuck_ssim (t: ctree E C X) (t': ctree F D Y):
+    is_stuck t -> ssim L t t'.
   Proof.
-    intros. step. now apply is_stuck_ss0.
+    intros. step. now apply is_stuck_ss.
   Qed.
 
-  Lemma stuckD_ss0 (R : rel _ _) (t : ctree F D Y) : ss0 L R stuckD t.
+  Lemma stuckD_ss (R : rel _ _) (t : ctree F D Y) : ss L R stuckD t.
   Proof.
     repeat intro. now apply stuckD_is_stuck in H.
   Qed.
 
-  Lemma stuckD_ssim0 (t : ctree F D Y) : ssim0 L stuckD t.
+  Lemma stuckD_ssim (t : ctree F D Y) : ssim L stuckD t.
   Proof.
-    intros. step. apply stuckD_ss0.
+    intros. step. apply stuckD_ss.
   Qed.
 
-  Lemma spinD_ss0 (R : rel _ _) (t : ctree F D Y) `{HasTau: B1 -< C}: ss0 L R spinD t.
+  Lemma spinD_ss (R : rel _ _) (t : ctree F D Y) `{HasTau: B1 -< C}: ss L R spinD t.
   Proof.
     repeat intro. now apply spinD_is_stuck in H.
   Qed.
 
-  Lemma spinD_ssim0 : forall (t' : ctree F D Y) `{HasTau: B1 -< C},
-      ssim0 L spinD t'.
+  Lemma spinD_ssim : forall (t' : ctree F D Y) `{HasTau: B1 -< C},
+      ssim L spinD t'.
   Proof.
-    intros. step. apply spinD_ss0.
+    intros. step. apply spinD_ss.
   Qed.
 
-End ssim0_heterogenous_theory.
+End ssim_heterogenous_theory.
 
 (*|
 Up-to [bind] context simulations
@@ -327,8 +327,8 @@ Section bind.
     Specialization of [bind_ctx] to a function acting with [ssim] on the bound value,
     and with the argument (pointwise) on the continuation.
     |*)
-  Program Definition bind_ctx_ssim0: mon (rel (ctree E C X') (ctree F D Y')) :=
-    {|body := fun R => @bind_ctx E F C D X Y X' Y' (ssim0 L) (pointwise (fun x y => L (val x) (val y)) R) |}.
+  Program Definition bind_ctx_ssim: mon (rel (ctree E C X') (ctree F D Y')) :=
+    {|body := fun R => @bind_ctx E F C D X Y X' Y' (ssim L) (pointwise (fun x y => L (val x) (val y)) R) |}.
   Next Obligation.
     intros ?? H. apply leq_bind_ctx. intros ?? H' ?? H''.
     apply in_bind_ctx. apply H'. intros t t' HS. apply H, H'', HS.
@@ -337,8 +337,8 @@ Section bind.
   (*|
     The resulting enhancing function gives a valid up-to technique
   |*)
-  Lemma bind_ctx_ssim0_t {RV: Respects_val L}:
-    bind_ctx_ssim0 <= (sst0 L).
+  Lemma bind_ctx_ssim_t {RV: Respects_val L}:
+    bind_ctx_ssim <= (sst L).
   Proof.
     apply Coinduction.
     intros R. apply (leq_bind_ctx _).
@@ -352,12 +352,12 @@ Section bind.
     apply trans_bind_l; eauto.
     + intro Hl. destruct Hl. apply RV in H0 as [_ ?]. specialize (H0 (Is_val _)). auto.
     + split; auto.
-        apply (fT_T equ_clos_sst0).
+        apply (fT_T equ_clos_sst).
         econstructor; [exact EQ | | reflexivity].
-        apply (fTf_Tf (ss0 L)).
+        apply (fTf_Tf (ss L)).
         apply in_bind_ctx; auto.
         intros ? ? ?.
-        apply (b_T (ss0 L)).
+        apply (b_T (ss L)).
         red in kk; cbn; now apply kk.
     + apply tt in STEPres as (u' & ? & STEPres & EQ' & ?).
       destruct RV.
@@ -370,7 +370,7 @@ Section bind.
       do 2 eexists; split.
       eapply trans_bind_r; eauto.
       split; auto.
-      eapply (id_T (ss0 L)); auto.
+      eapply (id_T (ss L)); auto.
   Qed.
 
 End bind.
@@ -378,16 +378,16 @@ End bind.
 (*|
 Expliciting the reasoning rule provided by the up-to principles.
 |*)
-Lemma sst0_clo_bind {E F C D: Type -> Type} {X Y X' Y': Type} {L: rel (@label E) (@label F)}
+Lemma sst_clo_bind {E F C D: Type -> Type} {X Y X' Y': Type} {L: rel (@label E) (@label F)}
       `{HasStuck: B0 -< C} `{HasStuck': B0 -< D} {RV: Respects_val L}
       (t1 : ctree E C X) (t2: ctree F D Y)
       (k1 : X -> ctree E C X') (k2 : Y -> ctree F D Y') RR:
-  ssim0 L t1 t2 ->
-  (forall x y, (sst0 L RR) (k1 x) (k2 y)) ->
-  sst0 L RR (t1 >>= k1) (t2 >>= k2).
+  ssim L t1 t2 ->
+  (forall x y, (sst L RR) (k1 x) (k2 y)) ->
+  sst L RR (t1 >>= k1) (t2 >>= k2).
 Proof.
   intros ? ?.
-  apply (ft_t (@bind_ctx_ssim0_t E F C D X X' Y Y' _ _ L RV)).
+  apply (ft_t (@bind_ctx_ssim_t E F C D X X' Y Y' _ _ L RV)).
   apply in_bind_ctx; eauto.
   intros ? ? ?; auto.
 Qed.
@@ -395,16 +395,16 @@ Qed.
 (*|
 Specializing the congruence principle for [≲]
 |*)
-Lemma ssim0_clo_bind {E F C D: Type -> Type} {X Y X' Y': Type}  {L: rel (@label E) (@label F)}
+Lemma ssim_clo_bind {E F C D: Type -> Type} {X Y X' Y': Type}  {L: rel (@label E) (@label F)}
       `{HasStuck: B0 -< C} `{HasStuck': B0 -< D} {RV: Respects_val L}
       (t1 : ctree E C X) (t2: ctree F D Y)
       (k1 : X -> ctree E C X') (k2 : Y -> ctree F D Y'):
-  ssim0 L t1 t2 ->
-  (forall x y, ssim0 L (k1 x) (k2 y)) ->
-  ssim0 L (t1 >>= k1) (t2 >>= k2).
+  ssim L t1 t2 ->
+  (forall x y, ssim L (k1 x) (k2 y)) ->
+  ssim L (t1 >>= k1) (t2 >>= k2).
 Proof.
   intros * EQ EQs.
-  apply (ft_t (@bind_ctx_ssim0_t E F C D X X' Y Y' _ _ L RV)).
+  apply (ft_t (@bind_ctx_ssim_t E F C D X X' Y Y' _ _ L RV)).
   apply in_bind_ctx; auto.
   intros ? ? ?; auto.
   apply EQs.
@@ -413,47 +413,47 @@ Qed.
 (*|
 And in particular, we can justify rewriting [≲] to the left of a [bind].
 |*)
-Lemma bind_ssim0_cong_gen {E C X X'} RR {HasStuck: B0 -< C}
+Lemma bind_ssim_cong_gen {E C X X'} RR {HasStuck: B0 -< C}
       {L: relation (@label E)} {RV: Respects_val L}:
-  Proper (ssim0 L ==> (fun f g => forall x y, sst0 L RR (f x) (g y)) ==> sst0 L RR) (@bind E C X X').
+  Proper (ssim L ==> (fun f g => forall x y, sst L RR (f x) (g y)) ==> sst L RR) (@bind E C X X').
 Proof.
   do 4 red; intros.
-  eapply sst0_clo_bind; auto.
+  eapply sst_clo_bind; auto.
 Qed.
 
-Ltac __upto_bind_ssim0 :=
+Ltac __upto_bind_ssim :=
   match goal with
-    |- @ssim0 ?E ?F ?C ?D ?X ?Y _ _ ?L (CTree.bind (T := ?T) _ _) (CTree.bind (T := ?T') _ _) =>
-      apply ssim0_clo_bind
-  | |- body (t (@ss0 ?E ?F ?C ?D ?X ?Y _ _ ?L)) ?R (CTree.bind (T := ?T) _ _) (CTree.bind (T := ?T') _ _) =>
-      apply (ft_t (@bind_ctx_ssim0_t E F C D X T Y T' _ L)), in_bind_ctx
-  | |- body (bt (@ss0 ?E ?F ?C ?D ?X ?Y _ _ ?L)) ?R (CTree.bind (T := ?T) _ _) (CTree.bind (T := ?T') _ _) =>
-      apply (fbt_bt (@bind_ctx_ssim0_t E F C D X T Y T' _ L)), in_bind_ctx
+    |- @ssim ?E ?F ?C ?D ?X ?Y _ _ ?L (CTree.bind (T := ?T) _ _) (CTree.bind (T := ?T') _ _) =>
+      apply ssim_clo_bind
+  | |- body (t (@ss ?E ?F ?C ?D ?X ?Y _ _ ?L)) ?R (CTree.bind (T := ?T) _ _) (CTree.bind (T := ?T') _ _) =>
+      apply (ft_t (@bind_ctx_ssim_t E F C D X T Y T' _ L)), in_bind_ctx
+  | |- body (bt (@ss ?E ?F ?C ?D ?X ?Y _ _ ?L)) ?R (CTree.bind (T := ?T) _ _) (CTree.bind (T := ?T') _ _) =>
+      apply (fbt_bt (@bind_ctx_ssim_t E F C D X T Y T' _ L)), in_bind_ctx
   end.
 
-Ltac __upto_bind_eq_ssim0 :=
+Ltac __upto_bind_eq_ssim :=
   match goal with
-  | |- @ssim0 ?E ?F ?C ?D ?X ?Y _ _ ?L (CTree.bind (T := ?T) _ _) (CTree.bind (T := ?T') _ _) =>
-      __upto_bind_ssim0; [reflexivity | intros ?]
-  | _ => __upto_bind_ssim0; [reflexivity | intros ? ? <-]
+  | |- @ssim ?E ?F ?C ?D ?X ?Y _ _ ?L (CTree.bind (T := ?T) _ _) (CTree.bind (T := ?T') _ _) =>
+      __upto_bind_ssim; [reflexivity | intros ?]
+  | _ => __upto_bind_ssim; [reflexivity | intros ? ? <-]
   end.
 
-Ltac __play_ssim0 := step; cbn; intros ? ? ?TR.
+Ltac __play_ssim := step; cbn; intros ? ? ?TR.
 
-Ltac __play_ssim0_in H :=
+Ltac __play_ssim_in H :=
   step in H;
   cbn in H; edestruct H as [? ?TR ?EQ];
   clear H; [etrans |].
 
-Ltac __eplay_ssim0 :=
+Ltac __eplay_ssim :=
   match goal with
-  | h : @ssim0 ?E ?F ?C ?D ?X ?Y _ _ ?L _ _ |- _ =>
-      __play_ssim0_in h
+  | h : @ssim ?E ?F ?C ?D ?X ?Y _ _ ?L _ _ |- _ =>
+      __play_ssim_in h
   end.
 
-#[local] Tactic Notation "play" := __play_ssim0.
-#[local] Tactic Notation "play" "in" ident(H) := __play_ssim0_in H.
-#[local] Tactic Notation "eplay" := __eplay_ssim0.
+#[local] Tactic Notation "play" := __play_ssim.
+#[local] Tactic Notation "play" "in" ident(H) := __play_ssim_in H.
+#[local] Tactic Notation "eplay" := __eplay_ssim.
 
 Section Proof_Rules.
 
@@ -462,11 +462,11 @@ Section Proof_Rules.
           {X : Type}
           {HasStuck: B0 -< C}.
 
-  Lemma step_ss0_ret_gen {Y F D} `{HasStuck': B0 -< D}(x : X) (y : Y) (R L : rel _ _) :
+  Lemma step_ss_ret_gen {Y F D} `{HasStuck': B0 -< D}(x : X) (y : Y) (R L : rel _ _) :
     R stuckD stuckD ->
     (Proper (equ eq ==> equ eq ==> impl) R) ->
     L (val x) (val y) ->
-    ss0 L R (Ret x : ctree E C X) (Ret y : ctree F D Y).
+    ss L R (Ret x : ctree E C X) (Ret y : ctree F D Y).
   Proof.
     intros Rstuck PROP Lval.
     cbn; intros ? ? TR; inv_trans; subst;
@@ -474,14 +474,14 @@ Section Proof_Rules.
       now rewrite EQ.
   Qed.
 
-  Lemma step_ss0_ret {Y F D} `{HasStuck': B0 -< D} (x : X) (y : Y) (R L : rel _ _) :
+  Lemma step_ss_ret {Y F D} `{HasStuck': B0 -< D} (x : X) (y : Y) (R L : rel _ _) :
     L (val x) (val y) ->
-    ssbt0 L R (Ret x : ctree E C X) (Ret y : ctree F D Y).
+    ssbt L R (Ret x : ctree E C X) (Ret y : ctree F D Y).
   Proof.
     intros.
-    apply step_ss0_ret_gen.
+    apply step_ss_ret_gen.
     - step. intros.
-      apply is_stuck_ss0; apply stuckD_is_stuck.
+      apply is_stuck_ss; apply stuckD_is_stuck.
     - typeclasses eauto.
     - apply H.
   Qed.
@@ -491,11 +491,11 @@ Section Proof_Rules.
     transition system, stepping is hence symmetric and we can just recover
     the itree-style rule.
   |*)
-  Lemma step_ss0_vis_gen {Y Z Z' F D} `{HasStuck': B0 -< D} (e : E Z) (f: F Z')
+  Lemma step_ss_vis_gen {Y Z Z' F D} `{HasStuck': B0 -< D} (e : E Z) (f: F Z')
         (k : Z -> ctree E C X) (k' : Z' -> ctree F D Y) (R L: rel _ _) :
     (Proper (equ eq ==> equ eq ==> impl) R) ->
     (forall x, exists y, R (k x) (k' y) /\ L (obs e x) (obs f y)) ->
-    ss0 L R (Vis e k) (Vis f k').
+    ss L R (Vis e k) (Vis f k').
   Proof.
     intros.
     cbn; intros ? ? TR; inv_trans; subst;
@@ -505,38 +505,38 @@ Section Proof_Rules.
     - assumption.
   Qed.
 
-  Lemma step_ss0_vis {Y Z F D} `{HasStuck': B0 -< D} (e : E Z) (f: F Z)
+  Lemma step_ss_vis {Y Z F D} `{HasStuck': B0 -< D} (e : E Z) (f: F Z)
         (k : Z -> ctree E C X) (k' : Z -> ctree F D Y) (R L : rel _ _) :
-    (forall x, exists y, sst0 L R (k x) (k' y) /\ L (obs e x) (obs f y)) ->
-    ssbt0 L R (Vis e k) (Vis f k').
+    (forall x, exists y, sst L R (k x) (k' y) /\ L (obs e x) (obs f y)) ->
+    ssbt L R (Vis e k) (Vis f k').
   Proof.
     intros * EQ.
-    apply step_ss0_vis_gen; auto.
+    apply step_ss_vis_gen; auto.
     typeclasses eauto.
   Qed.
 
   (*|
     Same goes for visible tau nodes.
     |*)
-  Lemma step_ss0_step_gen {Y F D} `{HasTau: B1 -< C} `{HasStuck': B0 -< D} `{HasTau': B1 -< D}
+  Lemma step_ss_step_gen {Y F D} `{HasTau: B1 -< C} `{HasStuck': B0 -< D} `{HasTau': B1 -< D}
         (t : ctree E C X) (t': ctree F D Y) (R L: rel _ _):
     (Proper (equ eq ==> equ eq ==> impl) R) ->
     L tau tau ->
     (R t t') ->
-    ss0 L R (Step t) (Step t').
+    ss L R (Step t) (Step t').
   Proof.
     intros PR ? EQs.
     intros ? ? TR; inv_trans; subst.
     cbn; do 2 eexists; split; [etrans | split; [rewrite EQ; eauto|assumption]].
   Qed.
 
-  Lemma step_ss0_step {Y F D} `{HasStuck': B0 -< D} `{HasTau: B1 -< C} `{HasTau': B1 -< D}
+  Lemma step_ss_step {Y F D} `{HasStuck': B0 -< D} `{HasTau: B1 -< C} `{HasTau': B1 -< D}
         (t: ctree E C X) (t': ctree F D Y) (R L : rel _ _) :
-    (sst0 L R t t') ->
+    (sst L R t t') ->
     L tau tau ->
-    ssbt0 L R (Step t) (Step t').
+    ssbt L R (Step t) (Step t').
   Proof.
-    intros. apply step_ss0_step_gen; auto.
+    intros. apply step_ss_step_gen; auto.
     typeclasses eauto.
   Qed.
 
@@ -546,47 +546,47 @@ Section Proof_Rules.
     A useful special case is the one where the arity coincide and we simply use the identity
     in both directions. We can in this case have [n] rather than [2n] obligations.
     |*)
-  Lemma step_ss0_brS_gen {Z Z' Y F D} `{HasStuck': B0 -< D} (c : C Z) (d : D Z')
+  Lemma step_ss_brS_gen {Z Z' Y F D} `{HasStuck': B0 -< D} (c : C Z) (d : D Z')
         (k : Z -> ctree E C X) (k' : Z' -> ctree F D Y) (R L: rel _ _) :
     (Proper (equ eq ==> equ eq ==> impl) R) ->
     (forall x, exists y, R (k x) (k' y)) ->
     L tau tau ->
-    ss0 L R (BrS c k) (BrS d k').
+    ss L R (BrS c k) (BrS d k').
   Proof.
     intros PROP EQs ? ? ? TR; inv_trans; subst.
     destruct (EQs x) as [y HR].
     cbn; do 2 eexists; split; [etrans | split; [rewrite EQ; eauto|assumption]].
   Qed.
 
-  Lemma step_ss0_brS {Z Z' Y F} (c : C Z) (c' : C Z')
+  Lemma step_ss_brS {Z Z' Y F} (c : C Z) (c' : C Z')
         (k : Z -> ctree E C X) (k' : Z' -> ctree F C Y) (R L: rel _ _) :
-    (forall x, exists y, sst0 L R (k x) (k' y)) ->
+    (forall x, exists y, sst L R (k x) (k' y)) ->
     L tau tau ->
-    ssbt0 L R (BrS c k) (BrS c' k').
+    ssbt L R (BrS c k) (BrS c' k').
   Proof.
     intros.
-    apply step_ss0_brS_gen; auto.
+    apply step_ss_brS_gen; auto.
     typeclasses eauto.
   Qed.
 
-  Lemma step_ss0_brS_id_gen {Z Y D F} `{HasStuck': B0 -< D} (c : C Z) (d: D Z)
+  Lemma step_ss_brS_id_gen {Z Y D F} `{HasStuck': B0 -< D} (c : C Z) (d: D Z)
         (k: Z -> ctree E C X) (k': Z -> ctree F D Y)(R L : rel _ _) :
     (Proper (equ eq ==> equ eq ==> impl) R) ->
     (forall x, exists y, R (k x) (k' y)) ->
     L tau tau ->
-    ss0 L R (BrS c k) (BrS d k').
+    ss L R (BrS c k) (BrS d k').
   Proof.
-    intros; apply step_ss0_brS_gen; eauto.
+    intros; apply step_ss_brS_gen; eauto.
   Qed.
 
-  Lemma step_ss0_brS_id {Z Y F} (c : C Z)
+  Lemma step_ss_brS_id {Z Y F} (c : C Z)
         (k: Z -> ctree E C X) (k': Z -> ctree F C Y)(R L : rel _ _) :
-    (forall x, exists y, sst0 L R (k x) (k' y)) ->
+    (forall x, exists y, sst L R (k x) (k' y)) ->
     L tau tau ->
-    ssbt0 L R (BrS c k) (BrS c k').
+    ssbt L R (BrS c k) (BrS c k').
   Proof.
     intros.
-    apply step_ss0_brS_id_gen; eauto.
+    apply step_ss_brS_id_gen; eauto.
     typeclasses eauto.
   Qed.
 
@@ -594,10 +594,10 @@ Section Proof_Rules.
     For invisible nodes, the situation is different: we may kill them, but that execution
     cannot act as going under the guard.
     |*)
-  Lemma step_ss0_guard_gen {Y F D} `{HasStuck': B0 -< D} `{HasTau: B1 -< C} `{HasTau': B1 -< D}
+  Lemma step_ss_guard_gen {Y F D} `{HasStuck': B0 -< D} `{HasTau: B1 -< C} `{HasTau': B1 -< D}
         (t: ctree E C X) (t': ctree F D Y) (R L: rel _ _):
-    ss0 L R t t' ->
-    ss0 L R (Guard t) (Guard t').
+    ss L R t t' ->
+    ss L R (Guard t) (Guard t').
   Proof.
     intros EQ.
     intros ? ? TR; inv_trans; subst.
@@ -605,18 +605,18 @@ Section Proof_Rules.
     do 2 eexists; split; [etrans | split; trivial].
   Qed.
 
-  Lemma step_ss0_guard {Y F D} `{HasStuck': B0 -< D} `{HasTau: B1 -< C} `{HasTau': B1 -< D}
+  Lemma step_ss_guard {Y F D} `{HasStuck': B0 -< D} `{HasTau: B1 -< C} `{HasTau': B1 -< D}
         (t: ctree E C X) (t': ctree F D Y) (R L: rel _ _):
-    ssbt0 L R t t' ->
-    ssbt0 L R (Guard t) (Guard t').
+    ssbt L R t t' ->
+    ssbt L R (Guard t) (Guard t').
   Proof.
-    apply step_ss0_guard_gen.
+    apply step_ss_guard_gen.
   Qed.
 
-  Lemma step_ss0_brD_l_gen {Y F D Z} `{HasStuck': B0 -< D} (c : C Z)
+  Lemma step_ss_brD_l_gen {Y F D Z} `{HasStuck': B0 -< D} (c : C Z)
         (k : Z -> ctree E C X) (t': ctree F D Y) (R L: rel _ _):
-    (forall x, ss0 L R (k x) t') ->
-    ss0 L R (BrD c k) t'.
+    (forall x, ss L R (k x) t') ->
+    ss L R (BrD c k) t'.
   Proof.
     intros EQs.
     intros ? ? TR; inv_trans; subst.
@@ -624,67 +624,67 @@ Section Proof_Rules.
     eauto.
   Qed.
 
-  Lemma step_ss0_brD_l {Y F D Z} `{HasStuck': B0 -< D} (c : C Z)
+  Lemma step_ss_brD_l {Y F D Z} `{HasStuck': B0 -< D} (c : C Z)
         (k : Z -> ctree E C X) (t: ctree F D Y) (R L: rel _ _):
-    (forall x, ssbt0 L R (k x) t) ->
-    ssbt0 L R (BrD c k) t.
+    (forall x, ssbt L R (k x) t) ->
+    ssbt L R (BrD c k) t.
   Proof.
-    apply step_ss0_brD_l_gen.
+    apply step_ss_brD_l_gen.
   Qed.
 
-  Lemma step_ss0_brD_r_gen {Y F D Z} `{HasStuck': B0 -< D} (c : D Z) x
+  Lemma step_ss_brD_r_gen {Y F D Z} `{HasStuck': B0 -< D} (c : D Z) x
         (k : Z -> ctree F D Y) (t: ctree E C X) (R L: rel _ _):
-    ss0 L R t (k x) ->
-    ss0 L R t (BrD c k).
+    ss L R t (k x) ->
+    ss L R t (BrD c k).
   Proof.
     cbn. intros.
     apply H in H0 as (? & ? & ? & ? & ?).
     exists x0; etrans.
   Qed.
 
-  Lemma step_ss0_brD_r{Y F D Z} `{HasStuck': B0 -< D} (c : D Z) x
+  Lemma step_ss_brD_r{Y F D Z} `{HasStuck': B0 -< D} (c : D Z) x
         (k : Z -> ctree F D Y) (t: ctree E C X) (R L: rel _ _):
-    ssbt0 L R t (k x) ->
-    ssbt0 L R t (BrD c k).
+    ssbt L R t (k x) ->
+    ssbt L R t (BrD c k).
   Proof.
-    intros. eapply step_ss0_brD_r_gen. apply H.
+    intros. eapply step_ss_brD_r_gen. apply H.
   Qed.
 
-  Lemma step_ss0_brD_gen {Y F D n m} `{HasStuck': B0 -< D} (a: C n) (b: D m)
+  Lemma step_ss_brD_gen {Y F D n m} `{HasStuck': B0 -< D} (a: C n) (b: D m)
     (k : n -> ctree E C X) (k' : m -> ctree F D Y) (R L : rel _ _) :
-    (forall x, exists y, ss0 L R (k x) (k' y)) ->
-    ss0 L R (BrD a k) (BrD b k').
+    (forall x, exists y, ss L R (k x) (k' y)) ->
+    ss L R (BrD a k) (BrD b k').
   Proof.
     intros EQs.
-    apply step_ss0_brD_l_gen.
+    apply step_ss_brD_l_gen.
     intros. destruct (EQs x) as [x' ?].
-    now apply step_ss0_brD_r_gen with (x:=x').
+    now apply step_ss_brD_r_gen with (x:=x').
   Qed.
 
-  Lemma step_ss0_brD {Y F D n m} `{HasStuck': B0 -< D} (cn: C n) (cm: D m)
+  Lemma step_ss_brD {Y F D n m} `{HasStuck': B0 -< D} (cn: C n) (cm: D m)
     (k : n -> ctree E C X) (k' : m -> ctree F D Y) (L R : rel _ _) :
-    (forall x, exists y, ssbt0 L R (k x) (k' y)) ->
-    ssbt0 L R (BrD cn k) (BrD cm k').
+    (forall x, exists y, ssbt L R (k x) (k' y)) ->
+    ssbt L R (BrD cn k) (BrD cm k').
   Proof.
-    apply step_ss0_brD_gen.
+    apply step_ss_brD_gen.
   Qed.
 
-  Lemma step_ss0_brD_id_gen {Y F D n m} `{HasStuck': B0 -< D} (c: C n) (d: D m)
+  Lemma step_ss_brD_id_gen {Y F D n m} `{HasStuck': B0 -< D} (c: C n) (d: D m)
         (k : n -> ctree E C X) (k' : m -> ctree F D Y)
         (R L : rel _ _) :
-    (forall x, exists y, ss0 L R (k x) (k' y)) ->
-    ss0 L R (BrD c k) (BrD d k').
+    (forall x, exists y, ss L R (k x) (k' y)) ->
+    ss L R (BrD c k) (BrD d k').
   Proof.
-   intros; apply step_ss0_brD_gen.
+   intros; apply step_ss_brD_gen.
     intros x; destruct (H x) as [y ?]; exists y; apply H0.
   Qed.
 
-  Lemma step_ss0_brD_id {Y F D n m} `{HasStuck': B0 -< D} (c: C n) (d: D m)
+  Lemma step_ss_brD_id {Y F D n m} `{HasStuck': B0 -< D} (c: C n) (d: D m)
     (k : n -> ctree E C X) (k': m -> ctree F D Y) (R L: rel _ _) :
-    (forall x, exists y, ssbt0 L R (k x) (k' y)) ->
-    ssbt0 L R (BrD c k) (BrD d k').
+    (forall x, exists y, ssbt L R (k x) (k' y)) ->
+    ssbt L R (BrD c k) (BrD d k').
   Proof.
-    apply step_ss0_brD_id_gen.
+    apply step_ss_brD_id_gen.
   Qed.
 
   (*|
@@ -697,7 +697,7 @@ Section Proof_Rules.
   Lemma spinS_gen_nonempty : forall {Z Y D F} {L: rel (label E) (label F)} `{HasStuck': B0 -< D}
                                (c: C X) (c': C Y) (x: X) (y: Y),
       L tau tau ->
-      ssim0 L (@spinS_gen E C Z X c) (@spinS_gen F C Z Y c').
+      ssim L (@spinS_gen E C Z X c) (@spinS_gen F C Z Y c').
   Proof.
     intros until L.
     coinduction S CIH; simpl; intros ? ? ? ? ? ? ? ? TR;
@@ -715,8 +715,8 @@ Section Proof_Rules.
     Inversion principles
     --------------------
     |*)
-  Lemma ssim0_ret_inv {F D} {L: rel (label E) (label F)} `{HasStuck': B0 -< D} (r1 r2 : X) :
-    ssim0 L (Ret r1 : ctree E C X) (Ret r2 : ctree F D X) ->
+  Lemma ssim_ret_inv {F D} {L: rel (label E) (label F)} `{HasStuck': B0 -< D} (r1 r2 : X) :
+    ssim L (Ret r1 : ctree E C X) (Ret r2 : ctree F D X) ->
     L (val r1) (val r2).
   Proof.
     intro.
@@ -725,9 +725,9 @@ Section Proof_Rules.
     inv_trans; subst; assumption.
   Qed.
 
-  Lemma ssim0_vis_inv_type {D Y X1 X2} {L: relation (label E)} `{HasStuck': B0 -< D}
+  Lemma ssim_vis_inv_type {D Y X1 X2} {L: relation (label E)} `{HasStuck': B0 -< D}
         (e1 : E X1) (e2 : E X2) (k1 : X1 -> ctree E C X) (k2 : X2 -> ctree E D Y) (x : X1):
-    ssim0 L (Vis e1 k1) (Vis e2 k2) ->
+    ssim L (Vis e1 k1) (Vis e2 k2) ->
     X1 = X2.
   Proof.
     intros.
@@ -737,10 +737,10 @@ Section Proof_Rules.
     instantiate (1:=x) in H0.
   Admitted.
 
-  Lemma ssbt0_vis_inv {F D Y X1 X2} {L: rel (label E) (label F)} `{HasStuck': B0 -< D}
+  Lemma ssbt_vis_inv {F D Y X1 X2} {L: rel (label E) (label F)} `{HasStuck': B0 -< D}
         (e1 : E X1) (e2 : F X2) (k1 : X1 -> ctree E C X) (k2 : X2 -> ctree F D Y) (x : X1) R:
-    ssbt0 L R (Vis e1 k1) (Vis e2 k2) ->
-    (exists y, L (obs e1 x) (obs e2 y))  /\ (forall x, exists y, sst0 L R (k1 x) (k2 y)).
+    ssbt L R (Vis e1 k1) (Vis e2 k2) ->
+    (exists y, L (obs e1 x) (obs e2 y))  /\ (forall x, exists y, sst L R (k1 x) (k2 y)).
   Proof.
     intros.
     split; intros; edestruct H as [? ? ?];
@@ -750,10 +750,10 @@ Section Proof_Rules.
     - now apply H1.
   Qed.
 
-  Lemma ssim0_vis_inv {F D Y X1 X2} {L: rel (label E) (label F)} `{HasStuck': B0 -< D}
+  Lemma ssim_vis_inv {F D Y X1 X2} {L: rel (label E) (label F)} `{HasStuck': B0 -< D}
         (e1 : E X1) (e2 : F X2) (k1 : X1 -> ctree E C X) (k2 : X2 -> ctree F D Y) (x : X1):
-    ssim0 L (Vis e1 k1) (Vis e2 k2) ->
-    (exists y, L (obs e1 x) (obs e2 y)) /\ (forall x, exists y, ssim0 L (k1 x) (k2 y)).
+    ssim L (Vis e1 k1) (Vis e2 k2) ->
+    (exists y, L (obs e1 x) (obs e2 y)) /\ (forall x, exists y, ssim L (k1 x) (k2 y)).
   Proof.
     intros.
     split.
@@ -769,10 +769,10 @@ Section Proof_Rules.
         apply IN.
   Qed.
 
-  Lemma ssim0_brS_inv {F D Y} {L: rel (label E) (label F)} `{HasStuck': B0 -< D}
+  Lemma ssim_brS_inv {F D Y} {L: rel (label E) (label F)} `{HasStuck': B0 -< D}
         n m (cn: C n) (cm: D m) (k1 : n -> ctree E C X) (k2 : m -> ctree F D Y) :
-    ssim0 L (BrS cn k1) (BrS cm k2) ->
-    (forall i1, exists i2, ssim0 L (k1 i1) (k2 i2)).
+    ssim L (BrS cn k1) (BrS cm k2) ->
+    (forall i1, exists i2, ssim L (k1 i1) (k2 i2)).
   Proof.
     intros EQ i1.
     eplay.
@@ -781,10 +781,10 @@ Section Proof_Rules.
     eexists; eauto.
   Qed.
 
-  Lemma ss0_brD_l_inv {F D Y} {L: rel (label E) (label F)} `{HasStuck': B0 -< D}
+  Lemma ss_brD_l_inv {F D Y} {L: rel (label E) (label F)} `{HasStuck': B0 -< D}
         n (c: C n) (t : ctree F D Y) (k : n -> ctree E C X) R:
-    ss0 L R (BrD c k) t ->
-    forall x, ss0 L R (k x) t.
+    ss L R (BrD c k) t ->
+    forall x, ss L R (k x) t.
   Proof.
     cbn. intros.
     eapply trans_brD in H0; [| reflexivity].
@@ -792,20 +792,20 @@ Section Proof_Rules.
     eauto.
   Qed.
 
-  Lemma ssim0_brD_l_inv {F D Y} {L: rel (label E) (label F)} `{HasStuck': B0 -< D}
+  Lemma ssim_brD_l_inv {F D Y} {L: rel (label E) (label F)} `{HasStuck': B0 -< D}
         n (c: C n) (t : ctree F D Y) (k : n -> ctree E C X):
-    ssim0 L (BrD c k) t ->
-    forall x, ssim0 L (k x) t.
+    ssim L (BrD c k) t ->
+    forall x, ssim L (k x) t.
   Proof.
-    intros. step. step in H. eapply ss0_brD_l_inv. apply H.
+    intros. step. step in H. eapply ss_brD_l_inv. apply H.
   Qed.
 
   (* This one isn't very convenient... *)
-  Lemma ssim0_brD_r_inv {F D Y} {L: rel (label E) (label F)} `{HasStuck': B0 -< D}
+  Lemma ssim_brD_r_inv {F D Y} {L: rel (label E) (label F)} `{HasStuck': B0 -< D}
         n (c: D n) (t : ctree E C X) (k : n -> ctree F D Y):
-    ssim0 L t (BrD c k) ->
+    ssim L t (BrD c k) ->
     forall l t', trans l t t' ->
-    exists l' x t'' , trans l' (k x) t'' /\ L l l' /\ (ssim0 L t' t'').
+    exists l' x t'' , trans l' (k x) t'' /\ L l l' /\ (ssim L t' t'').
   Proof.
     cbn. intros. step in H. apply H in H0 as (? & ? & ? & ? & ?); subst. inv_trans.
     do 3 eexists; eauto.
@@ -820,10 +820,10 @@ This property is true if we only allow brs with 0 or 1 branch,
 but we prove a counter-example for a ctree with a binary br.
 |*)
 
-Lemma ss0_sb : forall {E C X} RR {HasStuck: B0 -< C}
+Lemma ss_sb : forall {E C X} RR {HasStuck: B0 -< C}
   (t t' : ctree E C X),
-  ss0 eq RR t t' ->
-  ss0 eq (flip RR) t' t ->
+  ss eq RR t t' ->
+  ss eq (flip RR) t' t ->
   sb eq RR t t'.
 Proof.
   intros.
@@ -840,17 +840,17 @@ Qed.
 #[local] Definition t2 : ctree void1 (B0 +' B1 +' B2) unit :=
   brS2 (Ret tt) (stuckD).
 
-Lemma ssim0_sbisim_nequiv :
-  ssim0 eq t1 t2 /\ ssim0 eq t2 t1 /\ ~ sbisim eq t1 t2.
+Lemma ssim_sbisim_nequiv :
+  ssim eq t1 t2 /\ ssim eq t2 t1 /\ ~ sbisim eq t1 t2.
 Proof.
   unfold t1, t2. intuition.
   - step.
-    apply step_ss0_brS; auto.
+    apply step_ss_brS; auto.
     intros _. exists true. reflexivity.
-  - step. apply step_ss0_brS; auto.
+  - step. apply step_ss_brS; auto.
     intros [|]; exists tt.
     + reflexivity.
-    + step. apply stuckD_ss0.
+    + step. apply stuckD_ss.
   - step in H. cbn in H. destruct H as [_ ?].
     specialize (H tau stuckD). lapply H; [| etrans].
     intros. destruct H0 as (? & ? & ? & ? & ?).
