theories/Eq/SSimTheory.v
@@ -41,41 +41,41 @@ Arguments trans : simpl never.
   - Polymorphic on labels, by heterogenous relation [L].
   - Polymorphic on return type.
   - Polymorphic on branch effects. |*)
-Section ssim_heterogenous_theory.
-  
+Section cssim_heterogenous_theory.
+
   Arguments label: clear implicits.
   Context {E F C D: Type -> Type} {X Y: Type}
           {L: rel (@label E) (@label F)}
           {HasStuck1: B0 -< C} {HasStuck2: B0 -< D}.
-  
-  Notation ss0 := (@ss0 E F C D X Y _ _).
+
   Notation ss := (@ss E F C D X Y _ _).
-  Notation ssim  := (@ssim E F C D X Y _ _).
-  Notation sst L := (coinduction.t (ss L)).
-  Notation ssbt L := (coinduction.bt (ss L)).
-  Notation ssT L := (coinduction.T (ss L)).
+  Notation css := (@css E F C D X Y _ _).
+  Notation cssim  := (@cssim E F C D X Y _ _).
+  Notation csst L := (coinduction.t (css L)).
+  Notation cssbt L := (coinduction.bt (css L)).
+  Notation cssT L := (coinduction.T (css L)).
 
   (*|
     Various results on reflexivity and transitivity.
     |*)
-  Lemma sbisim_clos_ss : @sbisim_clos E F C D X Y _ _ eq eq <= (sst L).
+  Lemma sbisim_clos_css : @sbisim_clos E F C D X Y _ _ eq eq <= (csst L).
   Proof.
     intro R1. apply Coinduction.
-    cbn; intros Rs x y [z x' y' z' SBzx' [x'y' y'x'] SBy'z']; split. 
-    - intros l t zt.      
+    cbn; intros Rs x y [z x' y' z' SBzx' [x'y' y'x'] SBy'z']; split.
+    - intros l t zt.
       step in SBzx'.
       apply SBzx' in zt as (l' & t' & x't' & ? & ?); subst.
       destruct (x'y' _ _ x't') as (l'' & t'' & y't'' & ? & ?).
-      
+
       step in SBy'z'.
       apply SBy'z' in y't'' as (ll & tt & z'tt & ? & ?); subst.
       exists ll, tt; split; trivial.
       + split; trivial.
-        apply (f_Tf (ss L)).
+        apply (f_Tf (css L)).
         econstructor; eauto.
     - intros l t z't.
       step in SBy'z'.
-      symmetry in SBy'z'.      
+      symmetry in SBy'z'.
       apply SBy'z' in z't as (l' & t' & y't' & ? & ?); subst.
       destruct (y'x' _ _ y't') as (l'' & t'' & y't'' & ?).
       step in SBzx'.
@@ -88,9 +88,9 @@ Section ssim_heterogenous_theory.
     Aggressively providing instances for rewriting hopefully faster
     [sbisim] under all [ss1]-related contexts (consequence of the transitivity
     of the companion).
-  |*)    
-  #[global] Instance sbisim_clos_ssim_goal:
-    Proper (sbisim eq ==> sbisim eq ==> flip impl) (ssim L).
+  |*)
+  #[global] Instance sbisim_clos_cssim_goal:
+    Proper (sbisim eq ==> sbisim eq ==> flip impl) (cssim L).
   Proof.
     cbn.
     coinduction R CH. intros.
@@ -104,46 +104,46 @@ Section ssim_heterogenous_theory.
       split; [| assumption].
       symmetry in H7. eapply CH; eassumption.
     - step in H0; apply H0 in H2 as (? & ? & ? & ? & ?).
-      step in H1. apply H1 in H2 as (? & ? & ? & ?). 
+      step in H1. apply H1 in H2 as (? & ? & ? & ?).
       step in H. apply H in H5 as (? & ? & ? & ? & ?); simpl in *; subst.
       exists x3, x6.
       split; assumption.
   Qed.
 
-  #[global] Instance sbisim_clos_ssim_ctx :
-    Proper (sbisim eq ==> sbisim eq ==> impl) (ssim L).
+  #[global] Instance sbisim_clos_cssim_ctx :
+    Proper (sbisim eq ==> sbisim eq ==> impl) (cssim L).
   Proof.
-    repeat intro. symmetry in H, H0. eapply sbisim_clos_ssim_goal; eauto.
+    repeat intro. symmetry in H, H0. eapply sbisim_clos_cssim_goal; eauto.
   Qed.
 
-  #[global] Instance sbisim_clos_sst_goal RR :
-    Proper (sbisim eq ==> sbisim eq ==> flip impl) (sst L RR).
+  #[global] Instance sbisim_clos_csst_goal RR :
+    Proper (sbisim eq ==> sbisim eq ==> flip impl) (csst L RR).
   Proof.
     cbn; intros ? ? eq1 ? ? eq2 H.
-    apply (ft_t sbisim_clos_ss). cbn.
+    apply (ft_t sbisim_clos_css). cbn.
     econstructor; eauto.
     now rewrite eq2.
   Qed.
 
-  #[global] Instance sbisim_clos_sst_ctx RR :
-    Proper (sbisim eq ==> sbisim eq ==> impl) (sst L RR).
+  #[global] Instance sbisim_clos_csst_ctx RR :
+    Proper (sbisim eq ==> sbisim eq ==> impl) (csst L RR).
   Proof.
     cbn; intros ? ? eq1 ? ? eq2 ?.
     rewrite <- eq1, <- eq2.
     auto.
   Qed.
 
-  #[global] Instance sbisim_clos_ssT_goal RR f :
-    Proper (sbisim eq ==> sbisim eq ==> flip impl) (ssT L f RR).
+  #[global] Instance sbisim_clos_cssT_goal RR f :
+    Proper (sbisim eq ==> sbisim eq ==> flip impl) (cssT L f RR).
   Proof.
     cbn; intros ? ? eq1 ? ? eq2 H.
-    apply (fT_T sbisim_clos_ss). cbn.
+    apply (fT_T sbisim_clos_css). cbn.
     econstructor; eauto.
     now rewrite eq2.
   Qed.
 
-  #[global] Instance sbisim_clos_ssT_ctx RR f :
-    Proper (sbisim eq ==> sbisim eq ==> impl) (ssT L f RR).
+  #[global] Instance sbisim_clos_ccssT_ctx RR f :
+    Proper (sbisim eq ==> sbisim eq ==> impl) (cssT L f RR).
   Proof.
     cbn; intros ? ? eq1 ? ? eq2 ?.
     rewrite <- eq1, <- eq2.
@@ -154,7 +154,7 @@ Section ssim_heterogenous_theory.
     Strong simulation up-to [equ] is valid
     ----------------------------------------
     |*)
-  Lemma equ_clos_ss : equ_clos <= t (ss L).
+  Lemma equ_clos_css : equ_clos <= t (css L).
   Proof.
     apply Coinduction.
     intros R t u EQ; split; intros l ? TR; cbn in EQ; inv EQ;
@@ -164,139 +164,139 @@ Section ssim_heterogenous_theory.
         destruct TR as (? & ? & ? & ? & ?); subst;
         exists x, x0; intuition.
       + rewrite <- Equu; auto.
-      + eapply (f_Tf (ss L)).
+      + eapply (f_Tf (css L)).
         econstructor; auto; auto.
     - rewrite <- Equu in TR;
         apply HR in TR as (? & ? & ? & ?); subst;
         exists x, x0; intuition; rewrite Equt; auto.
   Qed.
 
-  #[global] Instance equ_clos_sst_goal RR :
-    Proper (equ eq ==> equ eq ==> flip impl) (sst L RR).
+  #[global] Instance equ_clos_csst_goal RR :
+    Proper (equ eq ==> equ eq ==> flip impl) (csst L RR).
   Proof.
     cbn; intros ? ? eq1 ? ? eq2 H.
-    apply (ft_t equ_clos_ss); econstructor; [eauto | | symmetry; eauto]; assumption.
+    apply (ft_t equ_clos_css); econstructor; [eauto | | symmetry; eauto]; assumption.
   Qed.
 
-  #[global] Instance equ_clos_sst_ctx RR :
-    Proper (equ eq ==> equ eq ==> impl) (sst L RR).
+  #[global] Instance equ_clos_csst_ctx RR :
+    Proper (equ eq ==> equ eq ==> impl) (csst L RR).
   Proof.
     cbn; intros ? ? eq1 ? ? eq2 H.
-    apply (ft_t equ_clos_ss); econstructor; [symmetry; eauto | | eauto]; assumption.
+    apply (ft_t equ_clos_css); econstructor; [symmetry; eauto | | eauto]; assumption.
   Qed.
 
-  #[global] Instance equ_ssbt_closed_goal {r}:
-    Proper (equ eq ==> equ eq ==> flip impl) (ssbt L r).
+  #[global] Instance equ_cssbt_closed_goal {r}:
+    Proper (equ eq ==> equ eq ==> flip impl) (cssbt L r).
   Proof.
     cbn; repeat intro.
     symmetry in H.
-    apply (fbt_bt equ_clos_ss); econstructor; [symmetry; eauto | | eauto].
-    apply (fbt_bt equ_clos_ss); econstructor; [reflexivity| eauto| eauto].
+    apply (fbt_bt equ_clos_css); econstructor; [symmetry; eauto | | eauto].
+    apply (fbt_bt equ_clos_css); econstructor; [reflexivity| eauto| eauto].
     now symmetry in H0.
   Qed.
 
-  #[global] Instance equ_ssbt_closed_ctx {r} :
-    Proper (equ eq ==> equ eq ==> impl) (ssbt L r).
+  #[global] Instance equ_cssbt_closed_ctx {r} :
+    Proper (equ eq ==> equ eq ==> impl) (cssbt L r).
   Proof.
-    cbn; repeat intro. 
+    cbn; repeat intro.
     setoid_rewrite H in H1. setoid_rewrite H0 in H1.
     auto.
   Qed.
 
-  #[global] Instance equ_clos_ssT_goal RR f :
-    Proper (equ eq ==> equ eq ==> flip impl) (ssT L f RR).
+  #[global] Instance equ_clos_cssT_goal RR f :
+    Proper (equ eq ==> equ eq ==> flip impl) (cssT L f RR).
   Proof.
     cbn; intros ? ? eq1 ? ? eq2 H.
-    apply (fT_T equ_clos_ss); econstructor; [eauto | | symmetry; eauto]; assumption.
+    apply (fT_T equ_clos_css); econstructor; [eauto | | symmetry; eauto]; assumption.
   Qed.
 
-  #[global] Instance equ_clos_ssT_ctx RR f :
-    Proper (equ eq ==> equ eq ==> impl) (ssT L f RR).
+  #[global] Instance equ_clos_cssT_ctx RR f :
+    Proper (equ eq ==> equ eq ==> impl) (cssT L f RR).
   Proof.
     cbn; intros ? ? eq1 ? ? eq2 H.
-    apply (fT_T equ_clos_ss); econstructor; [symmetry; eauto | | eauto]; assumption.
+    apply (fT_T equ_clos_css); econstructor; [symmetry; eauto | | eauto]; assumption.
   Qed.
 
-  #[global] Instance equ_clos_ssim_goal :
-    Proper (equ eq ==> equ eq ==> flip impl) (ssim L).
+  #[global] Instance equ_clos_cssim_goal :
+    Proper (equ eq ==> equ eq ==> flip impl) (cssim L).
   Proof.
     cbn; intros ? ? eq1 ? ? eq2 H.
-    apply (ft_t equ_clos_ss); econstructor; [eauto | | symmetry; eauto]; assumption.
+    apply (ft_t equ_clos_css); econstructor; [eauto | | symmetry; eauto]; assumption.
   Qed.
 
-  #[global] Instance equ_clos_ssim_ctx :
-    Proper (equ eq ==> equ eq ==> impl) (ssim L).
+  #[global] Instance equ_clos_cssim_ctx :
+    Proper (equ eq ==> equ eq ==> impl) (cssim L).
   Proof.
     cbn; intros ? ? eq1 ? ? eq2 H.
-    apply (ft_t equ_clos_ss); econstructor; [symmetry; eauto | | eauto]; assumption.
+    apply (ft_t equ_clos_css); econstructor; [symmetry; eauto | | eauto]; assumption.
   Qed.
 
-  #[global] Instance equ_ss_closed_goal {r} : Proper (equ eq ==> equ eq ==> flip impl) (ss L r).
+  #[global] Instance equ_css_closed_goal {r} : Proper (equ eq ==> equ eq ==> flip impl) (css L r).
   Proof.
     intros t t' tt' u u' uu'; cbn; intros [H H0]; split; intros l t0 TR.
-    - rewrite tt' in TR. destruct (H _ _ TR) as (? & ? & ? & ? & ?).     
+    - rewrite tt' in TR. destruct (H _ _ TR) as (? & ? & ? & ? & ?).
       exists x, x0; auto; rewrite uu'; auto.
     - rewrite uu' in TR. destruct (H0 _ _ TR) as (? & ? & ? & ?).
       exists x, x0; eauto; rewrite tt'; auto.
   Qed.
 
-  #[global] Instance equ_ss_closed_ctx {r} : Proper (equ eq ==> equ eq ==> impl) (ss L r).
+  #[global] Instance equ_css_closed_ctx {r} : Proper (equ eq ==> equ eq ==> impl) (css L r).
   Proof.
     intros t t' tt' u u' uu'; cbn; intros [H H0]; split; intros l t0 TR.
     - rewrite <- tt' in TR. destruct (H _ _ TR) as (? & ? & ? & ? & ?).
       exists x, x0; auto; rewrite <- uu'; auto.
-    - rewrite <- uu' in TR. destruct (H0 _ _ TR) as (? & ? & ? & ?). 
+    - rewrite <- uu' in TR. destruct (H0 _ _ TR) as (? & ? & ? & ?).
       exists x, x0; auto; rewrite <- tt'; auto.
   Qed.
 
-  Lemma is_stuck_ss : forall (t: ctree E C X) (u: ctree F D Y) R,
-      ss L R t u -> is_stuck t <-> is_stuck u.
+  Lemma is_stuck_css : forall (t: ctree E C X) (u: ctree F D Y) R,
+      css L R t u -> is_stuck t <-> is_stuck u.
   Proof.
     split; intros; intros ? ? ?.
     - apply H in H1 as (? & ? & ? & ?). now apply H0 in H2.
     - apply H in H1 as (? & ? & ? & ? & ?). now apply H0 in H1.
   Qed.
 
-  Lemma is_stuck_ssim :  forall (t: ctree E C X) (u: ctree F D Y),
+  Lemma is_stuck_cssim :  forall (t: ctree E C X) (u: ctree F D Y),
       t (⪅ L) u -> is_stuck t <-> is_stuck u.
   Proof.
-    intros. step in H. eapply is_stuck_ss; eauto.
+    intros. step in H. eapply is_stuck_css; eauto.
   Qed.
 
-  Lemma ss_is_stuck : forall (t : ctree E C X) (u: ctree F D Y) R,
-      is_stuck t -> is_stuck u -> ss L R t u.
+  Lemma css_is_stuck : forall (t : ctree E C X) (u: ctree F D Y) R,
+      is_stuck t -> is_stuck u -> css L R t u.
   Proof.
     split; intros.
     - cbn. intros. now apply H in H1.
     - now apply H0 in H1.
   Qed.
 
-  Lemma ssim_is_stuck : forall (t : ctree E C X) (u: ctree F D Y),
+  Lemma cssim_is_stuck : forall (t : ctree E C X) (u: ctree F D Y),
       is_stuck t -> is_stuck u -> t (⪅ L) u.
   Proof.
-    intros. step. now apply ss_is_stuck.
+    intros. step. now apply css_is_stuck.
   Qed.
 
-End ssim_heterogenous_theory.
+End cssim_heterogenous_theory.
 
-Section ssim_homogenous_theory.
+Section cssim_homogenous_theory.
 
   Context {E C : Type -> Type} {X : Type}
           {L: relation (@label E)}
           {HasStuck: B0 -< C}.
 
-  Notation ss0 := (@ss0 E E C C X X _ _).
   Notation ss := (@ss E E C C X X _ _).
-  Notation ssim  := (@ssim E E C C X X _ _).
-  Notation sst L := (coinduction.t (ss L)).
-  Notation ssbt L := (coinduction.bt (ss L)).
-  Notation ssT L := (coinduction.T (ss L)).
+  Notation css := (@css E E C C X X _ _).
+  Notation cssim  := (@cssim E E C C X X _ _).
+  Notation csst L := (coinduction.t (css L)).
+  Notation cssbt L := (coinduction.bt (css L)).
+  Notation cssT L := (coinduction.T (css L)).
 
-  Lemma ssim_subrelation : forall (t t' : ctree E C X) L',
-      subrelation L L' -> ssim L t t' -> ssim L' t t'.
+  Lemma cssim_subrelation : forall (t t' : ctree E C X) L',
+      subrelation L L' -> cssim L t t' -> cssim L' t t'.
   Proof.
     intros. revert t t' H0. coinduction R CH.
-    intros. step in H0. simpl; split; intros; cbn in H0; destruct H0 as [H0' H0''].  
+    intros. step in H0. simpl; split; intros; cbn in H0; destruct H0 as [H0' H0''].
     - cbn in H0'; apply H0' in H1 as (? & ? & ? & ? & ?);
         apply H in H2. exists x, x0. auto.
     - cbn in H0''; apply H0'' in H1 as (? & ? & ? & ?).
@@ -306,26 +306,25 @@ Section ssim_homogenous_theory.
   (*|
     Various results on reflexivity and transitivity.
     |*)
-  Lemma refl_sst `{Reflexive _ L}: const seq <= (sst L).
+  Lemma refl_csst `{Reflexive _ L}: const seq <= (csst L).
   Proof.
     intros. apply leq_t.
     cbn. intros. unfold seq in H0. subst. split; eauto.
   Qed.
 
-  #[global] Instance Reflexive_ss R `{Reflexive _ L} `{Reflexive _ R}: Reflexive (ss L R).
+  #[global] Instance Reflexive_ss R `{Reflexive _ L} : Reflexive (csst L R).
   Proof.
-    intros t.
-    split; simpl; intros l t' TR; exists l, t'; auto.
+    apply build_reflexive, ft_t, refl_csst.
   Qed.
 
-  #[global] Instance Reflexive_ssim `{Reflexive _ L}: Reflexive (ssim L).
+  #[global] Instance Reflexive_cssim `{Reflexive _ L}: Reflexive (cssim L).
   Proof.
     cbn.  coinduction R CH.
     intros t.
     split; simpl; intros l t' TR; exists l, t'; split; auto.
   Qed.
 
-  Lemma square_sst `{Transitive _ L}: square <= (sst L).
+  Lemma square_csst `{Transitive _ L}: square <= (csst L).
   Proof.
     apply Coinduction; cbn.
     intros R x z [y [xy yx] [yz zy]].
@@ -335,18 +334,19 @@ Section ssim_homogenous_theory.
       destruct (yz _ _ yy') as (l'' & z' & zz' & ? & ?).
       exists l'', z'.
       split; [assumption |split].
-      + apply (f_Tf (ss L)).
+      + apply (f_Tf (css L)).
         exists y'; eauto.
       + transitivity l'; auto.
     - intros l z' zz'.
-      destruct (zy _ _ zz') as (l' & y' & ? & yy'). 
+      destruct (zy _ _ zz') as (l' & y' & ? & yy').
       destruct (yx _ _ yy') as (l'' & x' & ? & xx').
       exists l'', x'.
       split; eauto with trans.
   Qed.
 
-  Lemma Transitive_ss R `{Transitive _ L} `{Transitive _ R}: Transitive (ss L R).
+  Lemma Transitive_ss R `{Transitive _ L} `{Transitive _ R}: Transitive (css L R).
   Proof.
+
     cbn.
     intros x y z [xy yx] [yz zy].
     split.
@@ -358,7 +358,7 @@ Section ssim_homogenous_theory.
       + now transitivity y'.
       + now transitivity l'.
     - intros l z' zz'.
-      destruct (zy _ _ zz') as (l' & y' & ? & yy'). 
+      destruct (zy _ _ zz') as (l' & y' & ? & yy').
       destruct (yx _ _ yy') as (l'' & x' & ? & xx').
       exists l'', z'.
       split.
@@ -366,19 +366,19 @@ Section ssim_homogenous_theory.
       + admit. (* LEF: not sure why this doesn't work *)
   Admitted.
 
-  #[global] Instance PreOrder_sst R `{PreOrder _ L}: PreOrder (sst L R).
-  Proof. apply PreOrder_t. apply refl_sst. apply square_sst. Qed.
+  #[global] Instance PreOrder_csst R `{PreOrder _ L}: PreOrder (csst L R).
+  Proof. apply PreOrder_t. apply refl_csst. apply square_csst. Qed.
 
-  Corollary PreOrder_ssim `{PreOrder _ L}:  PreOrder (ssim L).
-  Proof. now apply PreOrder_sst. Qed.
+  Corollary PreOrder_cssim `{PreOrder _ L}:  PreOrder (cssim L).
+  Proof. now apply PreOrder_csst. Qed.
 
-  #[global] Instance PreOrder_ssbt R `{PreOrder _ L}: PreOrder (ssbt L R).
-  Proof. apply rel.PreOrder_bt. now apply refl_sst. apply square_sst. Qed.
+  #[global] Instance PreOrder_cssbt R `{PreOrder _ L}: PreOrder (cssbt L R).
+  Proof. apply rel.PreOrder_bt. now apply refl_csst. apply square_csst. Qed.
 
-  #[global] Instance PreOrder_ssT f R `{PreOrder _ L}: PreOrder ((T (ss L)) f R).
-  Proof. apply rel.PreOrder_T. now apply refl_sst. apply square_sst. Qed.
+  #[global] Instance PreOrder_cssT f R `{PreOrder _ L}: PreOrder ((T (css L)) f R).
+  Proof. apply rel.PreOrder_T. now apply refl_csst. apply square_csst. Qed.
 
-End ssim_homogenous_theory.
+End cssim_homogenous_theory.
 
 (*|
 Up-to [bind] context simulations
@@ -397,11 +397,11 @@ Section bind.
           (L : hrel (@label E) (@label F)).
 
   (*|
-    Specialization of [bind_ctx] to a function acting with [ssim] on the bound value,
+    Specialization of [bind_ctx] to a function acting with [cssim] on the bound value,
     and with the argument (pointwise) on the continuation.
     |*)
-  Program Definition bind_ctx_ssim : mon (rel (ctree E C X') (ctree F D Y')) :=
-    {|body := fun R => @bind_ctx E F C D X Y X' Y' (ssim L) (pointwise (fun x y => L (val x) (val y)) R) |}.
+  Program Definition bind_ctx_cssim : mon (rel (ctree E C X') (ctree F D Y')) :=
+    {|body := fun R => @bind_ctx E F C D X Y X' Y' (cssim L) (pointwise (fun x y => L (val x) (val y)) R) |}.
   Next Obligation.
     intros ?? H. apply leq_bind_ctx. intros ?? H' ?? H''.
     apply in_bind_ctx. apply H'. intros t t' HS. apply H, H'', HS.
@@ -410,14 +410,14 @@ Section bind.
 (*|
 The resulting enhancing function gives a valid up-to technique
 |*)
-  Lemma bind_ctx_ssim_t {HL: Respects_val L}:
-    bind_ctx_ssim <= sst L.
+  Lemma bind_ctx_cssim_t {HL: Respects_val L}:
+    bind_ctx_cssim <= csst L.
   Proof.
     apply Coinduction.
     intros R. apply (leq_bind_ctx _).
     intros t1 t2 tt k1 k2 kk.
     step in tt.
-    split; simpl; intros l u STEP; 
+    split; simpl; intros l u STEP;
       apply trans_bind_inv in STEP as [(H & t' & STEP & EQ) | (v & STEPres & STEP)];
       cbn in *.
     - apply tt in STEP as (u' & l' & STEP & EQ' & ?).
@@ -425,26 +425,26 @@ The resulting enhancing function gives a valid up-to technique
       apply trans_bind_l; eauto.
       + intro Hl. destruct Hl. apply HL in H0 as [_ ?]. specialize (H0 (Is_val _)). auto.
       + split; auto.
-        apply (fT_T equ_clos_ss).
+        apply (fT_T equ_clos_css).
         econstructor; [exact EQ | | reflexivity].
-        apply (fTf_Tf (ss L)).
+        apply (fTf_Tf (css L)).
         apply in_bind_ctx; auto.
         intros ? ? ?.
-        apply (b_T (ss L)).
-        red in kk; now apply kk. 
+        apply (b_T (css L)).
+        red in kk; now apply kk.
     - apply tt in STEPres as (u' & ? & STEPres & EQ' & ?).
       destruct HL.
       pose proof (respects_val _ _ H) as [? _]. specialize (H0 (Is_val _)). destruct H0.
       pose proof (trans_val_invT STEPres). subst.
       pose proof (trans_val_inv STEPres) as EQ.
       rewrite EQ in STEPres.
-      specialize (kk v x0 H). 
+      specialize (kk v x0 H).
       apply kk in STEP as (u'' & ? & STEP & EQ'' & ?); cbn in *.
       do 2 eexists; split.
       eapply trans_bind_r; eauto.
       split; auto.
-      eapply (id_T (ss L)); auto.
-    - apply tt in STEP as (u' & l' & ? & STEP). 
+      eapply (id_T (css L)); auto.
+    - apply tt in STEP as (u' & l' & ? & STEP).
       do 2 eexists; split; eauto.
       apply trans_bind_l.
       + intro Hl. destruct Hl. apply HL in H0 as [? _]. specialize (H0 (Is_val _)). auto.
@@ -456,40 +456,40 @@ The resulting enhancing function gives a valid up-to technique
       pose proof (trans_val_invT STEPres). subst.
       pose proof (trans_val_inv STEPres) as EQ.
       rewrite EQ in STEPres.
-      specialize (kk x0 v H). 
+      specialize (kk x0 v H).
       apply kk in STEP as (u'' & ? & ? & STEP); cbn in *.
-      do 2 eexists; split; eauto.      
+      do 2 eexists; split; eauto.
       eapply trans_bind_r; eauto.
   Qed.
 
 End bind.
 
 (*| More lemmas about [bind] |*)
-Lemma bind_ctx_ssim_eq_t {E C T X} `{B0 -< C} :
-  (bind_ctx_ssim (X := T) (Y := T) eq : mon (relation (ctree E C X))) <= sst eq.
+Lemma bind_ctx_cssim_eq_t {E C T X} `{B0 -< C} :
+  (bind_ctx_cssim (X := T) (Y := T) eq : mon (relation (ctree E C X))) <= csst eq.
 Proof.
-  apply bind_ctx_ssim_t. split. intros. now subst.
+  apply bind_ctx_cssim_t. split. intros. now subst.
 Qed.
 
 (*|
 Expliciting the reasoning rule provided by the up-to principles.
 |*)
-Lemma sst_clo_bind {E F C D: Type -> Type} `{B0 -< C} `{B0 -< D}
+Lemma csst_clo_bind {E F C D: Type -> Type} `{B0 -< C} `{B0 -< D}
       {X X' Y Y' : Type} {L: rel (@label E) (@label F)} {HL: Respects_val L} (t1 : ctree E C X) (t2 : ctree F D X')
       (k1 : X -> ctree E C Y) (k2 : X' -> ctree F D Y') RR:
 		t1 (⪅ L) t2 ->
-    (forall x y, L (val x) (val y) -> (sst L RR) (k1 x) (k2 y)) ->
-    sst L RR (t1 >>= k1) (t2 >>= k2).
+    (forall x y, L (val x) (val y) -> (csst L RR) (k1 x) (k2 y)) ->
+    csst L RR (t1 >>= k1) (t2 >>= k2).
 Proof.
   intros.
-  apply (ft_t (@bind_ctx_ssim_t E F C D X Y X' Y' _ _ L HL)).
+  apply (ft_t (@bind_ctx_cssim_t E F C D X Y X' Y' _ _ L HL)).
   apply in_bind_ctx; auto.
 Qed.
 
 (*|
 Specializing the congruence principle for [~]
 |*)
-Lemma ssim_clo_bind {E F C D: Type -> Type} `{B0 -< C} `{B0 -< D}
+Lemma cssim_clo_bind {E F C D: Type -> Type} `{B0 -< C} `{B0 -< D}
       {X X' Y Y' : Type} L {HL: Respects_val L} (t1 : ctree E C X) (t2 : ctree F D X')
       (k1 : X -> ctree E C Y) (k2 : X' -> ctree F D Y'):
 		t1 (⪅L) t2 ->
@@ -498,64 +498,64 @@ Lemma ssim_clo_bind {E F C D: Type -> Type} `{B0 -< C} `{B0 -< D}
 .
 Proof.
   intros.
-  apply (ft_t (@bind_ctx_ssim_t E F C D X Y X' Y' _ _ L HL)).
+  apply (ft_t (@bind_ctx_cssim_t E F C D X Y X' Y' _ _ L HL)).
   apply in_bind_ctx; auto.
 Qed.
 
 (*|
 And in particular, we can justify rewriting [⪅] to the left of a [bind].
 |*)
-Lemma bind_ssim_cong_gen {E F C D X X' Y Y'} `{B0 -< C} `{B0 -< D} RR (L : rel _ _)
+Lemma bind_cssim_cong_gen {E F C D X X' Y Y'} `{B0 -< C} `{B0 -< D} RR (L : rel _ _)
       {HL: Respects_val L} (t : ctree E C X) (t' : ctree F D X')
       (k : X -> ctree E C Y) (k' : X' -> ctree F D Y'):
-    ssim L t t' ->
-    (forall x x', L (val x) (val x') -> sst L RR (k x) (k' x')) ->
-    sst L RR (CTree.bind t k) (CTree.bind t' k').
+    cssim L t t' ->
+    (forall x x', L (val x) (val x') -> csst L RR (k x) (k' x')) ->
+    csst L RR (CTree.bind t k) (CTree.bind t' k').
 Proof.
-  intros; eapply sst_clo_bind; red in H2; eauto.
+  intros; eapply csst_clo_bind; red in H2; eauto.
 Qed.
 
-(*| Ltac automation rule for [bind] and [ssim] |*)
-Ltac __upto_bind_ssim :=
+(*| Ltac automation rule for [bind] and [cssim] |*)
+Ltac __upto_bind_cssim :=
   match goal with
-    |- @ssim _ _ _ _ ?X ?X' _ _ _ (CTree.bind (T := ?T) _ _) (CTree.bind (T := ?T') _ _) =>
-      apply ssim_clo_bind
-  | |- body (t (@ss ?E ?E ?C ?C ?X ?X _ _ eq)) ?R (CTree.bind (T := ?T) _ _) (CTree.bind (T := ?T) _ _) =>
-      apply (ft_t (@bind_ctx_ssim_eq_t E C T X _)), in_bind_ctx
-  | |- body (bt (@ss ?E ?E ?C ?C ?X ?X _ _ eq)) ?R (CTree.bind (T := ?T) _ _) (CTree.bind (T := ?T) _ _) =>
-      apply (fbt_bt (@bind_ctx_ssim_eq_t E C T X _)), in_bind_ctx
+    |- @cssim _ _ _ _ ?X ?X' _ _ _ (CTree.bind (T := ?T) _ _) (CTree.bind (T := ?T') _ _) =>
+      apply cssim_clo_bind
+  | |- body (t (@css ?E ?E ?C ?C ?X ?X _ _ eq)) ?R (CTree.bind (T := ?T) _ _) (CTree.bind (T := ?T) _ _) =>
+      apply (ft_t (@bind_ctx_cssim_eq_t E C T X _)), in_bind_ctx
+  | |- body (bt (@css ?E ?E ?C ?C ?X ?X _ _ eq)) ?R (CTree.bind (T := ?T) _ _) (CTree.bind (T := ?T) _ _) =>
+      apply (fbt_bt (@bind_ctx_cssim_eq_t E C T X _)), in_bind_ctx
   end.
 
-Ltac __upto_bind_eq_ssim :=
-  __upto_bind_ssim; [reflexivity | intros ? _ _].
+Ltac __upto_bind_eq_cssim :=
+  __upto_bind_cssim; [reflexivity | intros ? _ _].
 
-Ltac __play_ssim := step; cbn; intros ? ? ?TR.
+Ltac __play_cssim := step; cbn; intros ? ? ?TR.
 
-Ltac __play_ssim_in H :=
+Ltac __play_cssim_in H :=
   step in H;
   cbn in H; edestruct H as (? & ? & ? & ? & ? );
   clear H; subst; [etrans |].
 
-Ltac __eplay_ssim :=
+Ltac __eplay_cssim :=
   match goal with
-  | h : @ssim ?E ?F ?C ?D ?X ?Y _ _ ?L _ _ |- _ =>
-      __play_ssim_in h
+  | h : @cssim ?E ?F ?C ?D ?X ?Y _ _ ?L _ _ |- _ =>
+      __play_cssim_in h
   end.
 
-#[local] Tactic Notation "play" := __play_ssim.
-#[local] Tactic Notation "play" "in" ident(H) := __play_ssim_in H.
-#[local] Tactic Notation "eplay" := __eplay_ssim.
+#[local] Tactic Notation "play" := __play_cssim.
+#[local] Tactic Notation "play" "in" ident(H) := __play_cssim_in H.
+#[local] Tactic Notation "eplay" := __eplay_cssim.
 
 Section Proof_Rules.
   Arguments label: clear implicits.
   Context {E C : Type -> Type} {X: Type} `{HasStuck : B0 -< C}.
 
-  Lemma step_ss_ret_gen {Y F D}(x : X) (y : Y) `{HasStuck': B0 -< D}
+  Lemma step_css_ret_gen {Y F D}(x : X) (y : Y) `{HasStuck': B0 -< D}
         {L: rel (label E) (label F)} {R : rel (ctree E C X) (ctree F D Y)}:
     R stuckD stuckD ->
     (Proper (equ eq ==> equ eq ==> impl) R) ->
     L (val x) (val y) ->
-    ss L R (Ret x : ctree E C X) (Ret y : ctree F D Y).
+    css L R (Ret x : ctree E C X) (Ret y : ctree F D Y).
   Proof.
     intros Rstuck PROP Lval.
     cbn; split; intros ? ? TR; inv_trans; subst;
@@ -563,14 +563,14 @@ Section Proof_Rules.
       now rewrite EQ.
   Qed.
 
-  Lemma step_ss_ret  {Y F D}(x : X) (y : Y) `{HasStuck': B0 -< D}
+  Lemma step_css_ret  {Y F D}(x : X) (y : Y) `{HasStuck': B0 -< D}
         {L: rel (label E) (label F)} {R : rel (ctree E C X) (ctree F D Y)}:
     L (val x) (val y) ->
-    ssbt L R (Ret x : ctree E C X) (Ret y : ctree F D Y).
+    cssbt L R (Ret x : ctree E C X) (Ret y : ctree F D Y).
   Proof.
     intros.
-    apply step_ss_ret_gen.
-    - step. intros. apply ss_is_stuck; apply stuckD_is_stuck.
+    apply step_css_ret_gen.
+    - step. intros. apply css_is_stuck; apply stuckD_is_stuck.
     - typeclasses eauto.
     - apply H.
   Qed.
@@ -582,38 +582,38 @@ Section Proof_Rules.
   |*)
   (* LEF: Here, I got lazy -- it would be nice to have [k': Z' -> ctree F D Y]
      see [step_ss0_vis_gen] *)
-   Lemma step_ss_vis_gen {Y Z F D} `{HasStuck': B0 -< D} (e : E Z) (f: F Z)
+   Lemma step_css_vis_gen {Y Z F D} `{HasStuck': B0 -< D} (e : E Z) (f: F Z)
         (k : Z -> ctree E C X) (k' : Z -> ctree F D Y) (R L: rel _ _) :
     (Proper (equ eq ==> equ eq ==> impl) R) ->
     (forall x, R (k x) (k' x)) ->
     (forall x, L (obs e x) (obs f x)) ->
-    ss L R (Vis e k) (Vis f k').
+    css L R (Vis e k) (Vis f k').
   Proof.
     split.
-    - apply step_ss0_vis_gen; eauto.
+    - apply step_ss_vis_gen; eauto.
     - intros. inv_trans; subst; etrans.
   Qed.
 
-  Lemma step_ss_vis {Y Z F D} `{HasStuck': B0 -< D} (e : E Z) (f: F Z)
+  Lemma step_css_vis {Y Z F D} `{HasStuck': B0 -< D} (e : E Z) (f: F Z)
         (k : Z -> ctree E C X) (k' : Z -> ctree F D Y) (R L: rel _ _) :
-    (forall x, sst L R (k x) (k' x)) ->
+    (forall x, csst L R (k x) (k' x)) ->
     (forall x, L (obs e x) (obs f x)) ->
-    ssbt L R (Vis e k) (Vis f k').
+    cssbt L R (Vis e k) (Vis f k').
   Proof.
     intros * EQ.
-    apply step_ss_vis_gen; auto.
+    apply step_css_vis_gen; auto.
     typeclasses eauto.
   Qed.
-  
+
   (*|
     Same goes for visible tau nodes.
-  |*)  
+  |*)
   Lemma step_ss_step_gen{Y F D} `{HasStuck': B0 -< D} `{HasTau: B1 -< C} `{HasTau': B1 -< D}
         (t : ctree E C X) (t' : ctree F D Y) (R L: rel _ _) :
     (Proper (equ eq ==> equ eq ==> impl) R) ->
     (R t t') ->
     L tau tau ->
-    ss L R (Step t) (Step t').
+    css L R (Step t) (Step t').
   Proof.
     intros PR EQs ?.
     cbn; split; intros ? ? TR; inv_trans; subst;
@@ -622,11 +622,11 @@ Section Proof_Rules.
     - assumption.
   Qed.
 
-  Lemma step_ss_step{Y F D} `{HasStuck': B0 -< D} `{HasTau: B1 -< C} `{HasTau': B1 -< D}
+  Lemma step_css_step{Y F D} `{HasStuck': B0 -< D} `{HasTau: B1 -< C} `{HasTau': B1 -< D}
         (t : ctree E C X) (t' : ctree F D Y) (R L: rel _ _) :
     L tau tau ->
-    (sst L R t t') ->
-    ssbt L R (Step t) (Step t').
+    (csst L R t t') ->
+    cssbt L R (Step t) (Step t').
   Proof.
     intros. eapply step_ss_step_gen; eauto.
     typeclasses eauto.
@@ -649,50 +649,50 @@ Section Proof_Rules.
     L tau tau ->
     inhabited Z ->
     (forall x, exists y, R (k x) (k' y)) ->
-    ss L R (BrS c k) (BrS d k').
+    css L R (BrS c k) (BrS d k').
   Proof.
-    intros PROP ? EX EQs; cbn; split; 
+    intros PROP ? EX EQs; cbn; split;
       intros ? ? TR; inv_trans; subst.
     - destruct (EQs x) as [z HR].
-      do 2 eexists; intuition.      
+      do 2 eexists; intuition.
       rewrite EQ; eassumption.
     - exists tau; eexists; intuition.
       Unshelve. apply (proj1_sig EX).
   Qed.
 
-  Lemma step_ss_brS {Y Z Z' F D} `{HasStuck': B0 -< D} (c : C Z) (d: D Z')
+  Lemma step_css_brS {Y Z Z' F D} `{HasStuck': B0 -< D} (c : C Z) (d: D Z')
         (k : Z -> ctree E C X) (k' : Z' -> ctree F D Y) (R L: rel _ _) :
     L tau tau ->
     inhabited Z ->
-    (forall x, exists y, sst L R (k x) (k' y)) ->
-    ssbt L R (BrS c k) (BrS d k').
+    (forall x, exists y, csst L R (k x) (k' y)) ->
+    cssbt L R (BrS c k) (BrS d k').
   Proof.
     intros.
     apply step_ss_brS_gen; auto.
     typeclasses eauto.
   Qed.
 
-  Lemma step_ss_brS_id_gen {Y Z F } (c : C Z)
+  Lemma step_css_brS_id_gen {Y Z F } (c : C Z)
         (k : Z -> ctree E C X) (k' : Z -> ctree F C Y) (R L: rel _ _) :
     (Proper (equ eq ==> equ eq ==> impl) R) ->
     L tau tau ->
     inhabited Z ->
     (forall x, R (k x) (k' x)) ->
-    ss L R (BrS c k) (BrS c k').
+    css L R (BrS c k) (BrS c k').
   Proof.
     intros PROP ? ? EQs.
     apply step_ss_brS_gen; auto.
     intros x; exists x; auto.
   Qed.
 
-  Lemma step_ss_brS_id {Y Z F } (c : C Z)
+  Lemma step_css_brS_id {Y Z F } (c : C Z)
         (k : Z -> ctree E C X) (k' : Z -> ctree F C Y) (R L: rel _ _) :
     L tau tau ->
     inhabited Z ->
-    (forall x, sst L R (k x) (k' x)) ->
-    ssbt L R (BrS c k) (BrS c k').
+    (forall x, csst L R (k x) (k' x)) ->
+    cssbt L R (BrS c k) (BrS c k').
   Proof.
-    apply step_ss_brS_id_gen.
+    apply step_css_brS_id_gen.
     typeclasses eauto.
   Qed.
 
@@ -700,10 +700,10 @@ Section Proof_Rules.
     For invisible nodes, the situation is different: we may kill them, but that
     execution cannot act as going under the guard.
   |*)
-  Lemma step_ss_guard_gen {Y F D} `{HasStuck': B0 -< D}`{HasTau: B1 -< C} `{HasTau': B1 -< D}
+  Lemma step_css_guard_gen {Y F D} `{HasStuck': B0 -< D}`{HasTau: B1 -< C} `{HasTau': B1 -< D}
         (t : ctree E C X) (t' : ctree F D Y) (R L: rel _ _) :
-    ss L R t t' ->
-    ss L R (Guard t) (Guard t').
+    css L R t t' ->
+    css L R (Guard t) (Guard t').
   Proof.
     intros EQ; cbn; split; intros ? ? TR; inv_trans; subst.
     - apply EQ in TR as (? & ? & ? & ? & ?).
@@ -714,19 +714,19 @@ Section Proof_Rules.
       + apply trans_guard; eauto.
   Qed.
 
-  Lemma step_ss_guard {Y F D} `{HasStuck': B0 -< D}`{HasTau: B1 -< C} `{HasTau': B1 -< D}
+  Lemma step_css_guard {Y F D} `{HasStuck': B0 -< D}`{HasTau: B1 -< C} `{HasTau': B1 -< D}
         (t : ctree E C X) (t' : ctree F D Y) (R L : rel _ _) :
-    ssbt L R t t' ->
-    ssbt L R (Guard t) (Guard t').
+    cssbt L R t t' ->
+    cssbt L R (Guard t) (Guard t').
   Proof.
-    apply step_ss_guard_gen.
+    apply step_css_guard_gen.
   Qed.
 
-  Lemma step_ss_brD_l_gen {Y F D Z} `{HasStuck': B0 -< D} (c : C Z)
+  Lemma step_css_brD_l_gen {Y F D Z} `{HasStuck': B0 -< D} (c : C Z)
     (k : Z -> ctree E C X) (t' : ctree F D Y) (R L: rel _ _) :
-    (forall x, ss L R (k x) t') ->
-    inhabited Z -> 
-    ss L R (BrD c k) t'.
+    (forall x, css L R (k x) t') ->
+    inhabited Z ->
+    css L R (BrD c k) t'.
   Proof.
     intros EQs ?; cbn; split;
       intros ? ? TR; inv_trans; subst.
@@ -738,19 +738,19 @@ Section Proof_Rules.
       eapply trans_brD; eauto.
   Qed.
 
-  Lemma step_ss_brD_l {Y F D Z} `{HasStuck': B0 -< D} (c : C Z)
+  Lemma step_css_brD_l {Y F D Z} `{HasStuck': B0 -< D} (c : C Z)
     (k : Z -> ctree E C X) (t' : ctree F D Y) (R L: rel _ _) :
-    (forall x, ssbt L R (k x) t') ->
+    (forall x, cssbt L R (k x) t') ->
     inhabited Z ->
-    ssbt L R (BrD c k) t'.
+    cssbt L R (BrD c k) t'.
   Proof.
-    apply step_ss_brD_l_gen.
+    apply step_css_brD_l_gen.
   Qed.
 
-  Lemma step_ss_brD_r_gen {Y F D Z} `{HasStuck': B0 -< D} (c : D Z)
+  Lemma step_css_brD_r_gen {Y F D Z} `{HasStuck': B0 -< D} (c : D Z)
     (t : ctree E C X) (k : Z -> ctree F D Y) (R L: rel _ _) z :
-    ss L R t (k z) ->
-    ss L R t (BrD c k).
+    css L R t (k z) ->
+    css L R t (BrD c k).
   Proof.
     simpl. split; intros.
     - apply H in H0 as (? & ? & ? & ? & ?); subst.
@@ -760,52 +760,52 @@ Section Proof_Rules.
       admit.
   Admitted.
 
-  Lemma step_ss_brD_r {Y F D Z} `{HasStuck': B0 -< D} (c : D Z)
+  Lemma step_css_brD_r {Y F D Z} `{HasStuck': B0 -< D} (c : D Z)
         (t : ctree E C X) (k : Z -> ctree F D Y) (R L: rel _ _) z :
-    ssbt L R t (k z) ->
-    ssbt L R t (BrD c k).
+    cssbt L R t (k z) ->
+    cssbt L R t (BrD c k).
   Proof.
-    intros. eapply step_ss_brD_r_gen. apply H.
+    intros. eapply step_css_brD_r_gen. apply H.
   Qed.
 
-  Lemma step_ss_brD_gen {Y F D Z Z'} `{HasStuck': B0 -< D} (c: C Z) (c': D Z')
+  Lemma step_css_brD_gen {Y F D Z Z'} `{HasStuck': B0 -< D} (c: C Z) (c': D Z')
         (k : Z -> ctree E C X) (k' : Z' -> ctree F D Y) (R L: rel _ _) :
-    (forall x, exists y, ss L R (k x) (k' y)) ->
+    (forall x, exists y, css L R (k x) (k' y)) ->
     inhabited Z ->
-    ss L R (BrD c k) (BrD c' k').
+    css L R (BrD c k) (BrD c' k').
   Proof.
     intros EQs ?.
-    apply step_ss_brD_l_gen; trivial.
+    apply step_css_brD_l_gen; trivial.
     intros. destruct (EQs x) as [x' ?].
-    now apply step_ss_brD_r_gen with (z := x').
+    now apply step_css_brD_r_gen with (z := x').
   Qed.
 
-  Lemma step_ss_brD {Y F D Z Z'} `{HasStuck': B0 -< D} (c: C Z) (c': D Z')
+  Lemma step_css_brD {Y F D Z Z'} `{HasStuck': B0 -< D} (c: C Z) (c': D Z')
         (k : Z -> ctree E C X) (k' : Z' -> ctree F D Y) (R L: rel _ _) :
-    (forall x, exists y, ssbt L R (k x) (k' y)) ->
-    inhabited Z -> 
-    ssbt L R (BrD c k) (BrD c' k').
+    (forall x, exists y, cssbt L R (k x) (k' y)) ->
+    inhabited Z ->
+    cssbt L R (BrD c k) (BrD c' k').
   Proof.
-    apply step_ss_brD_gen.
+    apply step_css_brD_gen.
   Qed.
 
-  Lemma step_ss_brD_id_gen {Y F Z} (c: C Z)
+  Lemma step_css_brD_id_gen {Y F Z} (c: C Z)
         (k : Z -> ctree E C X) (k' : Z -> ctree F C Y) (R L: rel _ _) :
-    (forall x, ss L R (k x) (k' x)) ->
+    (forall x, css L R (k x) (k' x)) ->
     inhabited Z ->
-    ss L R (BrD c k) (BrD c k').
+    css L R (BrD c k) (BrD c k').
   Proof.
-    intros; apply step_ss_brD_gen; trivial.
+    intros; apply step_css_brD_gen; trivial.
     intros x; exists x; apply H.
   Qed.
 
-  Lemma step_ss_brD_id {Y F Z} (c: C Z)
+  Lemma step_css_brD_id {Y F Z} (c: C Z)
         (k : Z -> ctree E C X) (k' : Z -> ctree F C Y) (R L: rel _ _) :
-    (forall x, ssbt L R (k x) (k' x)) ->
-    inhabited Z -> 
-    ssbt L R (BrD c k) (BrD c k').
+    (forall x, cssbt L R (k x) (k' x)) ->
+    inhabited Z ->
+    cssbt L R (BrD c k) (BrD c k').
   Proof.
-    apply step_ss_brD_id_gen.
+    apply step_css_brD_id_gen.
   Qed.
 
 End Proof_Rules.
@@ -828,7 +828,7 @@ Section WithParams.
     |*)
   Lemma spinS_gen_nonempty : forall {Z Z' X Y} (c: C X) (c': D Y) (x: X) (y: Y) (L : rel _ _),
     L tau tau ->
-    ssim L (@spinS_gen E C Z X c) (@spinS_gen F D Z' Y c').
+    cssim L (@spinS_gen E C Z X c) (@spinS_gen F D Z' Y c').
   Proof.
     intros.
     red. coinduction R CH.
@@ -847,7 +847,7 @@ Section WithParams.
     Inversion principles
     --------------------
   |*)
-  Lemma ssim_ret_inv X Y (r1 : X) (r2 : Y) :
+  Lemma cssim_ret_inv X Y (r1 : X) (r2 : Y) :
     (Ret r1 : ctree E C X) (⪅L) (Ret r2 : ctree F D Y) ->
     L (val r1) (val r2).
   Proof.
@@ -855,7 +855,7 @@ Section WithParams.
     eplay. inv_trans. now subst.
   Qed.
 
-  Lemma ssim_vis_inv_type {X X1 X2}
+  Lemma cssim_vis_inv_type {X X1 X2}
         (e1 : E X1) (e2 : E X2) (k1 : X1 -> ctree E C X) (k2 : X2 -> ctree E C X) (x : X1):
     Vis e1 k1 ⪅ Vis e2 k2 ->
     X1 = X2.
@@ -867,10 +867,10 @@ Section WithParams.
     step in H1; inv H1; reflexivity.
     Unshelve. admit.
   Admitted.
-  
-  Lemma ssbt_eq_vis_inv {X Y} (e1 e2 : E Y) (k1 k2 : Y -> ctree E C X) (x : Y) R :
-    ss eq (t (ss eq) R) (Vis e1 k1) (Vis e2 k2) ->
-    e1 = e2 /\ forall x, sst eq R (k1 x) (k2 x).
+
+  Lemma cssbt_eq_vis_inv {X Y} (e1 e2 : E Y) (k1 k2 : Y -> ctree E C X) (x : Y) R :
+    css eq (t (css eq) R) (Vis e1 k1) (Vis e2 k2) ->
+    e1 = e2 /\ forall x, csst eq R (k1 x) (k2 x).
   Proof.
     intros.
     split.
@@ -887,20 +887,20 @@ Section WithParams.
     reflexivity.
   Qed.
 
-  Lemma ssim_eq_vis_inv {X Y} (e1 e2 : E Y) (k1 k2 : Y -> ctree E C X) (x : Y) :
+  Lemma cssim_eq_vis_inv {X Y} (e1 e2 : E Y) (k1 k2 : Y -> ctree E C X) (x : Y) :
     Vis e1 k1 ⪅ Vis e2 k2 ->
     e1 = e2 /\ forall x, k1 x ⪅ k2 x.
   Proof.
     intros.
     (* Why doesn't apply work directly here? *)
-    epose proof (proj1 (enhanced_gfp (@ss E E C C X X _ _ eq) _ _)). apply H0 in H. clear H0.
-    step in H. apply ssbt_eq_vis_inv in H; auto.
+    epose proof (proj1 (enhanced_gfp (@css E E C C X X _ _ eq) _ _)). apply H0 in H. clear H0.
+    step in H. apply cssbt_eq_vis_inv in H; auto.
     destruct H. split; auto.
     intro. subst. specialize (H0 x0).
-    apply (proj1 (t_gfp_bt (@ss E E C C X X _ _ eq) _ _)) in H0. apply H0.
+    apply (proj1 (t_gfp_bt (@css E E C C X X _ _ eq) _ _)) in H0. apply H0.
   Qed.
 
-  Lemma ssim_brS_inv {X Y Z Z'}
+  Lemma cssim_brS_inv {X Y Z Z'}
         c1 c2 (k1 : X -> ctree E C Z) (k2 : Y -> ctree F D Z') :
     BrS c1 k1 (⪅L) BrS c2 k2 ->
     (forall i1, exists i2, k1 i1 (⪅L) k2 i2).
@@ -909,12 +909,12 @@ Section WithParams.
     eplay.
     inv_trans;
       eexists; eauto.
-  Admitted.    
+  Admitted.
 
-  Lemma ss_brD_l_inv : forall {X Y Z}
+  Lemma css_brD_l_inv : forall {X Y Z}
     (t : ctree E C X) (c : D Y) (k : Y -> ctree F D Z) L R,
-    ss L R (BrD c k) t ->
-    forall x, ss L R (k x) t.
+    css L R (BrD c k) t ->
+    forall x, css L R (k x) t.
   Proof.
     cbn. intros; split; intros.
     eapply trans_brD in H0; [| reflexivity].
@@ -922,20 +922,20 @@ Section WithParams.
     - apply H in H0 as (? & ? & ? & ?). apply trans_brD_inv in H1 as (x' & y').
   Admitted.
 
-  Lemma ssim_brD_l_inv : forall {X Y Z}
+  Lemma cssim_brD_l_inv : forall {X Y Z}
     (t : ctree E C X) (c : D Y) (k : Y -> ctree F D Z) L,
     BrD c k (⪅L) t ->
     forall x, k x (⪅L) t.
   Proof.
-    intros. step. step in H. eapply ss_brD_l_inv. apply H.
+    intros. step. step in H. eapply css_brD_l_inv. apply H.
   Qed.
 
   (* This one isn't very convenient... *)
-  Lemma ssim_brD_r_inv : forall {X Y Z}
+  Lemma cssim_brD_r_inv : forall {X Y Z}
     (t : ctree E C X) (c : D Y) (k : Y -> ctree F D Z) L,
-    ssim L t (BrD c k) ->
+    cssim L t (BrD c k) ->
     forall l t', trans l t t' ->
-    exists x t'' l', trans l' (k x) t'' /\ ssim L t' t'' /\ L l l'.
+    exists x t'' l', trans l' (k x) t'' /\ cssim L t' t'' /\ L l l'.
   Proof.
     cbn. intros. step in H. apply H in H0 as (? & ? & ? & ? & ?). subst. inv_trans.
     exists x1, x0, x. auto.
@@ -950,10 +950,10 @@ This property is true if we only allow choices with 0 or 1 branch,
 but we prove a counter-example for a ctree with a binary choice.
 |*)
 
-Lemma ss_sb : forall {E F C D X Y} `{B0 -< C} `{B0 -< D} L RR
+Lemma css_sb : forall {E F C D X Y} `{B0 -< C} `{B0 -< D} L RR
   (t : ctree E C X) (t' : ctree F D Y),
-  ss L RR t t' ->
-  ss (flip L) (flip RR) t' t ->
+  css L RR t t' ->
+  css (flip L) (flip RR) t' t ->
   sb L RR t t'.
 Proof.
   split; cbn; intros.
@@ -976,14 +976,14 @@ Proof.
     now rewrite <- H, EQ.
   - subst. rewrite <- ctree_eta. now rewrite <- H, EQ.
   - rewrite EQ. apply br0_always_stuck.
-Qed. 
+Qed.
 
 
-Lemma ssim_sbisim_equiv_gen :
+Lemma cssim_sbisim_equiv_gen :
   forall {E F X Y} (L : rel _ _) `{Injective (@label E) (@label F) L}
     `{Deterministic _ _ L}
     (t : ctree E B01 X) (t' : ctree F B01 Y),
-  ssim L t t' -> ssim (flip L) t' t -> sbisim L t t'.
+  cssim L t t' -> cssim (flip L) t' t -> sbisim L t t'.
 Proof.
   intros until 2.
   coinduction R CH. red. red. cbn. split; intros.
@@ -1005,14 +1005,14 @@ Proof.
     + apply H5.
   Qed.
 
-Lemma ssim_sbisim_equiv_eq : forall {E X} (t t' : ctree E B01 X),
-  ssim eq t t' -> ssim eq t' t -> sbisim eq t t'.
+Lemma cssim_sbisim_equiv_eq : forall {E X} (t t' : ctree E B01 X),
+  cssim eq t t' -> cssim eq t' t -> sbisim eq t t'.
 Proof.
-  intros. apply ssim_sbisim_equiv_gen; intros.
-  - typeclasses eauto. 
+  intros. apply cssim_sbisim_equiv_gen; intros.
+  - typeclasses eauto.
   - typeclasses eauto.
   - apply H.
-  - apply (@ssim_subrelation _ _ _ eq); auto.
+  - apply (@cssim_subrelation _ _ _ eq); auto.
     red. intros. subst. reflexivity.
 Qed.
 
@@ -1022,18 +1022,18 @@ Qed.
 #[local] Definition t2 : ctree void1 (B01 +' B2) unit :=
   brS2 (Ret tt) (stuckD).
 
-Lemma ssim_sbisim_nequiv :
-  ssim eq t1 t2 /\ ssim (flip eq) t2 t1 /\ ~ sbisim eq t1 t2.
+Lemma cssim_sbisim_nequiv :
+  cssim eq t1 t2 /\ cssim (flip eq) t2 t1 /\ ~ sbisim eq t1 t2.
 Proof.
   unfold t1, t2. intuition.
-  - step. eapply step_ss_brS; auto.
+  - step. eapply step_css_brS; auto.
     exact  (exist _ tt I).
     intros _. exists true. reflexivity.
-  - step. eapply step_ss_brS; auto.
+  - step. eapply step_css_brS; auto.
     exact  (exist _ true I).
     intro. exists tt. destruct x.
     + reflexivity.
-    + step. apply ss_is_stuck.
+    + step. apply css_is_stuck.
       * apply stuckD_is_stuck.
       * admit. (* This looks wrong, Ret is not stuck *)
   - step in H. cbn in H. destruct H as [_ ?].
@@ -1044,4 +1044,3 @@ Proof.
     intro. destruct H1 as (? & ? & ? & ? & ?). subst.
     now apply stuckD_is_stuck in H1.
 Admitted.
-
